updated proofs for knowledge soundness in the AGM

KZG_BatchOpening_knowledge_soundness.thy
@@ -1,1013 +1,630 @@
 theory KZG_BatchOpening_knowledge_soundness
 
-imports KZG_BatchOpening_binding
+imports KZG_BatchOpening_binding Algebraic_Group_Model
 begin
 
-text \<open>We extend the knowledge soundness definiton from the KZG to the batched version.
-We show knowledge soundness oriented at the definition in the PLONK paper (see section 3.1
-in the PLONK paper: https://eprint.iacr.org/2019/953.pdf). However, we show the property only for 
-a commitment to one polynomial to stay consistent with the other proofs in this work. Due to the 
-layout of the property though, this proof should be easily extendable to multiple polynomials 
-and thus serve as a strong basis for a proof for the full PLONK version.\<close>
 
-locale knowledge_sound_game_def = bind_game_proof
-begin
+text \<open>In this theory we prove knowledge soundness for the KZG, concretely the knowledge soundness 
+as defined in the abstract polynomial commitment scheme. The proof is a reduction to the 
+evaluation binding game which has been reduced to the t-Bilinear strong Diffie-Hellmann problem in the 
+KZG_eval_bind theory.\<close>
 
-section \<open>Definitions for the knowledge soundness game\<close>
+hide_const restrict
 
-text \<open>We define the knowledge soundness game, the reduction to the evaluation binding game and thus 
-transitively to the t-BSDH assumption as well as any functions needed to construct them in this 
-locale. This file contains another locale below which contains the proof. The proof is analog to the 
-normal KZG knowledge soundness proof.\<close>
+locale BatchEvalKZG_PCS_knowledge_sound = BatchEvalKZG_PCS_binding
+begin 
 
-subsection \<open>Game definition\<close>
+text \<open>the AGM adversary types that are useful in defining reductions (i.e. the reduction to the 
+evaluation binding game)\<close>
+lift_to_algebraicT "('a ck, 'a commit, 'state) knowledge_soundness_adversary1"  "G\<^sub>p" 
+  => AGM_knowledge_soundness_adversary1
+lift_to_algebraicT "('state, 'a ck, 'e mod_ring, 'e evaluation, 'a witness) knowledge_soundness_adversary2" 
+  "G\<^sub>p"  => AGM_knowledge_soundness_adversary2
 
-text \<open>Note, the adversary for the knowledge soundness is in the Algebraic Group Model (AGM) and 
-thus has to provide a vector we typed `calc_vector` for every group element it outputs. Furthermore, 
-the group elements must be a linear combination of the group elements the adversary has seen so far.
-the vector indicates the parameters of the linear combination. Intuitively, for e.g.
-seen group elements (3,2,1), the adversary could create the value 5 with the vector (0,2,1) as 
-5 = 3*0+2*2+1*1.\<close>
-
-text \<open>Furthermore, the adversary for knowledge soundness is split up into two parts A=(A',A'') 
-that share a state, which we type \<sigma>.\<close>
-
-type_synonym '\<sigma>' state = '\<sigma>'
-
-type_synonym 'e' calc_vector = "'e' mod_ring list"
-
-type_synonym ('a', 'e', '\<sigma>')  adversary_1 = 
-  "'a' pk \<Rightarrow> 
- ('a' commit \<times> 'e' calc_vector \<times> '\<sigma>' state) spmf"
-
-type_synonym ('a', 'e', '\<sigma>')  adversary_2 = 
-  "'\<sigma>' state \<Rightarrow>'a' pk \<Rightarrow> 'a' commit \<Rightarrow> 'e' calc_vector \<Rightarrow> 
-   ('e' eval_position \<times> 'e' eval_position set\<times> 'e' polynomial \<times> 'a' eval_witness) spmf"
+text \<open>We adapt the knowledge soundness adversary in round 2 to the batch version. 
+Concretely, we aks the adversary to give a single point $i \in I$ at which the evaluation polynomial 
+$r$ is disticnt from the extractor polynomial\<close>
+type_synonym ('e', 'state', 'a') knowledge_soundness_adversary2_AGM 
+  = "('a' ck \<times> 'state') \<Rightarrow> ('e' mod_ring \<times> 'e' argument set \<times> ('e' batch_evaluation \<times> ('a' witness \<times> int list))) spmf"
 
 text \<open>The extractor is an algorithm that plays against the adversary. It is granted access to the 
 adversaries messages and state (which we neglect in this case as we do not need it because the 
 calculation vector is enough to create sensible values) and has to come up with a polynomial such 
 that the adversary cannot create valid opening points that are not part of the polynomial.\<close>
 type_synonym ('a', 'e') extractor = 
-  "'a' commit \<Rightarrow> 'e' calc_vector \<Rightarrow> 
-    'e' mod_ring poly"
+  "('a' commit \<times> int list) \<Rightarrow> 
+    ('e' mod_ring poly \<times> unit) spmf"
 
-text \<open>This is the formalized knowledge soundness game\<close>
-definition knowledge_soundness_game :: "('a, 'e) extractor \<Rightarrow> ('a, 'e, '\<sigma>) adversary_1 \<Rightarrow> ('a, 'e, '\<sigma>) adversary_2 
-  \<Rightarrow> bool spmf"
-  where "knowledge_soundness_game E \<A> \<A>' = TRY do {
-  PK \<leftarrow> KeyGen;
-  (C,calc_vec, \<sigma>) \<leftarrow> \<A> PK;
-  _ :: unit \<leftarrow> assert_spmf (length PK = length calc_vec 
-                          \<and> C = fold (\<lambda> i acc. acc \<otimes>\<^bsub>G\<^sub>p\<^esub> PK!i ^\<^bsub>G\<^sub>p\<^esub> (calc_vec!i)) [0..<length PK] \<one>\<^bsub>G\<^sub>p\<^esub>);  
-  let \<phi> = E C calc_vec;
-  (i, B, r_x, w_B) \<leftarrow> \<A>' \<sigma> PK C calc_vec;
-  _ ::unit \<leftarrow> assert_spmf (i \<in> B  \<and> valid_batch_msg r_x w_B B);
-  return_spmf (VerifyEvalBatch PK C B r_x w_B \<and> poly r_x i \<noteq> poly \<phi> i)} ELSE return_spmf False"
+text \<open>restrict for AGM adversaries 1 & 2\<close>
 
-text \<open>The advantage of the adversary over the knowledge soundness game is the probabillity that it 
-wins.\<close>
-definition knowledge_soundness_game_advantage :: "('a, 'e) extractor \<Rightarrow> ('a, 'e, '\<sigma>) adversary_1 \<Rightarrow> ('a, 'e, '\<sigma>) adversary_2 
-   \<Rightarrow> real"
-  where "knowledge_soundness_game_advantage E \<A> \<A>' \<equiv> spmf (knowledge_soundness_game E \<A> \<A>') True"
+interpretation AGM1: Algebraic_Algorithm G\<^sub>p "listS G\<^sub>p.groupS" "prodC G\<^sub>p.groupC noConstrain" 
+  by (unfold_locales)
 
-subsection \<open>reduction definition\<close>
+text \<open>"'ck' \<Rightarrow> 'state' \<Rightarrow> ('argument' \<times> ('evaluation' \<times> 'witness')) spmf"\<close>
+interpretation AGM2: Algebraic_Algorithm G\<^sub>p "prodS (listS G\<^sub>p.groupS) noSelect" 
+  "prodC noConstrain (prodC noConstrain (prodC noConstrain G\<^sub>p.groupC))"
+  by (unfold_locales)
 
-text \<open>The reduction function takes a adversary for the knowledge soundness game and returns an 
-adversary for the evaluation binding game. Specifically, the reduction uses the knowledge soundness 
-adversary to construct a winning strategy for the evaluation binding game (i.e. to win it every 
-time).
-Essentially, it uses the fact that the values supplied by the adversary already break the binding 
-game.\<close>
-definition knowledge_soundness_reduction
-  :: "('a, 'e) extractor \<Rightarrow> ('a, 'e, '\<sigma>) adversary_1 \<Rightarrow> ('a, 'e, '\<sigma>) adversary_2 \<Rightarrow> ('a, 'e) adversary"                     
-where
-  "knowledge_soundness_reduction E \<A> \<A>' PK = do {
-  (C,calc_vec, \<sigma>) \<leftarrow> \<A> PK; 
-  let \<phi> = E C calc_vec;
-  (i, B, r_x, w_B) \<leftarrow> \<A>' \<sigma> PK C calc_vec;
-  let \<phi>_i = poly \<phi> i;
-  let w_i = createWitness PK \<phi> i;
-  return_spmf (C, i, \<phi>_i, w_i, B, w_B, r_x)}"
+definition knowledge_soundness_game_AGM :: "('state, 'a) AGM_knowledge_soundness_adversary1  
+  \<Rightarrow> ('e, 'state, 'a) knowledge_soundness_adversary2_AGM \<Rightarrow> ('a, 'e) extractor \<Rightarrow> bool spmf"
+  where "knowledge_soundness_game_AGM \<A>1 \<A>2 \<E> = TRY do {
+      (ck,vk) \<leftarrow> key_gen;
+      ((c,cvec),\<sigma>) \<leftarrow> AGM1.restrict \<A>1 ck;
+      (p,td) \<leftarrow> \<E> (c,cvec);
+      (i, I, (r, (w, wvec))) \<leftarrow> AGM2.restrict \<A>2 (ck,\<sigma>);
+      let (p_i,w') = Eval ck td p i;        
+      return_spmf (verify_eval_batch vk c I (r,w) \<and> poly r i \<noteq> p_i 
+        \<and> valid_argument_batch I \<and> valid_eval_batch (r,w) \<and> i \<in> I)       
+    } ELSE return_spmf False"
 
-end
-
-text \<open>This locale captures the proof for the definitions provided earlier\<close>
-locale knowledge_sound_game_proof = knowledge_sound_game_def
-begin
-
-subsection \<open>helping definitions\<close>
-
-text \<open>The knowledge soundness reduction adversary extended for asserts that 
-are present in the evaluation binding game. We use this definition to show equivalence to 
-the evaluation binding game. Later on we can then easily over-estimate the probability from 
-this extended version to the normal reduction.\<close>
-definition knowledge_soundness_reduction_ext
-  :: "('a, 'e) extractor \<Rightarrow> ('a, 'e, '\<sigma>) adversary_1 \<Rightarrow> ('a, 'e, '\<sigma>) adversary_2 \<Rightarrow> ('a, 'e) adversary"                     
-where
-  "knowledge_soundness_reduction_ext E \<A> \<A>' PK = do {
-  (C,calc_vec, \<sigma>) \<leftarrow> \<A> PK;
-  _ :: unit \<leftarrow> assert_spmf (length PK = length calc_vec 
-                          \<and> C = fold (\<lambda> i acc. acc \<otimes>\<^bsub>G\<^sub>p\<^esub> PK!i ^\<^bsub>G\<^sub>p\<^esub> (calc_vec!i)) [0..<length PK] \<one>\<^bsub>G\<^sub>p\<^esub>);  
-  let \<phi> = E C calc_vec;
-  (i, B, r_x, w_B) \<leftarrow> \<A>' \<sigma> PK C calc_vec;
-  let \<phi>_i = poly \<phi> i;
-  let w_i = createWitness PK \<phi> i;
-  return_spmf (C, i, \<phi>_i, w_i, B, w_B, r_x)}"
+definition ks_to_eval_bind_reduction :: "('state, 'a) AGM_knowledge_soundness_adversary1  
+  \<Rightarrow> ('e, 'state, 'a) knowledge_soundness_adversary2_AGM \<Rightarrow> ('a, 'e) extractor 
+  \<Rightarrow> ('a, 'e)  adversary" where 
+  "ks_to_eval_bind_reduction \<A>1 \<A>2 \<E> ck = do {
+    ((c,cvec),\<sigma>) \<leftarrow> AGM1.restrict \<A>1 ck;
+      (p,td) \<leftarrow> \<E> (c,cvec);
+      (i, I, (r_x, (w, wvec))) \<leftarrow> AGM2.restrict \<A>2 (ck,\<sigma>);
+      let (p_i,w') = Eval ck td p i;    
+      return_spmf (c,i, p_i, w', I, w, r_x)
+  }"
 
 text \<open>Extractor definition\<close>
 fun E :: "('a, 'e) extractor" where 
-  "E C calc_vec = Poly calc_vec"
+  "E (c,cvec) = return_spmf (Poly (map (of_int_mod_ring::int \<Rightarrow>'e mod_ring) cvec),())"
 
-lemma key_gen_alt_def: "KeyGen = do {
-    x :: nat \<leftarrow> sample_uniform (order G\<^sub>p);
-    let \<alpha>::'e mod_ring = of_int_mod_ring (int x) in
-    return_spmf (map (\<lambda>t. \<^bold>g\<^bsub>G\<^sub>p\<^esub> ^\<^bsub>G\<^sub>p\<^esub> (\<alpha>^t)) [0..<max_deg+1])
-  }"
-  unfolding KeyGen_def Setup_def Let_def split_def by simp
-
-subsection \<open>literal helping lemmas\<close>
-
-lemma pull_down_assert_spmf_with_return:
-"do {
-    z::'z \<leftarrow> Z:: 'z spmf;
-    x::'x \<leftarrow> (X:: 'z \<Rightarrow> 'x spmf) z;
-    _ :: unit \<leftarrow> assert_spmf((f::'z \<Rightarrow> 'x \<Rightarrow> bool) z x);
-    y::'y \<leftarrow> (Y:: 'z \<Rightarrow> 'x \<Rightarrow> 'y spmf) z x;
-    _ :: unit \<leftarrow> assert_spmf ((A::'y \<Rightarrow> bool) y);
-    return_spmf ((g::'z \<Rightarrow> 'x \<Rightarrow> 'y \<Rightarrow> bool) z x y) }
-  = do {
-    z::'z \<leftarrow> Z:: 'z spmf;
-    x::'x \<leftarrow> (X:: 'z \<Rightarrow> 'x spmf) z;
-    y::'y \<leftarrow> (Y:: 'z \<Rightarrow> 'x \<Rightarrow> 'y spmf) z x;
-    _ :: unit \<leftarrow> assert_spmf((f::'z \<Rightarrow> 'x \<Rightarrow> bool) z x);
-    _ :: unit \<leftarrow> assert_spmf ((A::'y \<Rightarrow> bool) y);
-    return_spmf ((g::'z \<Rightarrow> 'x \<Rightarrow> 'y \<Rightarrow> bool) z x y) }"
+lemma reduction_map_imp: "
+       let ck = map (\<lambda>t. \<^bold>g\<^bsub>G\<^sub>p\<^esub> ^\<^bsub>G\<^sub>p\<^esub> (\<alpha>^t)) [0..<max_deg+1];
+           vk = map (\<lambda>t. \<^bold>g\<^bsub>G\<^sub>p\<^esub> ^\<^bsub>G\<^sub>p\<^esub> (\<alpha>^t)) [0..<max_deg+1];
+           (p_i,w_i) = Eval ck td (Poly (map (of_int_mod_ring::int \<Rightarrow>'e mod_ring) cvec)) i 
+       in
+        length ck = length cvec 
+        \<and> c = fold (\<lambda> i acc. acc \<otimes> ck!i [^] (cvec!i)) [0..<length ck] \<one> 
+        \<and> verify_eval_batch vk c I (r_x,w) \<and> poly r_x i \<noteq> p_i 
+        \<and> valid_argument_batch I \<and> valid_eval_batch (r_x,w) \<and> i \<in> I
+  \<longrightarrow> 
+        length ck = length cvec 
+        \<and> c = fold (\<lambda> i acc. acc \<otimes> ck!i [^] (cvec!i)) [0..<length ck] \<one> 
+        \<and> i \<in> I \<and> p_i \<noteq> poly r_x i 
+        \<and> valid_argument_batch I \<and> valid_eval (p_i, w_i) \<and> valid_eval_batch (r_x, w) 
+        \<and> verify_eval vk c i (p_i, w_i)
+        \<and> verify_eval_batch vk c I (r_x,w)"
 proof -
-  have "\<forall>z x. do {
-    _ :: unit \<leftarrow> assert_spmf((f::'z \<Rightarrow> 'x \<Rightarrow> bool) z x);
-    y::'y \<leftarrow> (Y:: 'z \<Rightarrow> 'x \<Rightarrow> 'y spmf) z x;
-    _ :: unit \<leftarrow> assert_spmf ((A::'y \<Rightarrow> bool) y);
-    return_spmf ((g::'z \<Rightarrow> 'x \<Rightarrow> 'y \<Rightarrow> bool) z x y) }
-  = do {
-    y::'y \<leftarrow> (Y:: 'z \<Rightarrow> 'x \<Rightarrow> 'y spmf) z x;
-    _ :: unit \<leftarrow> assert_spmf((f::'z \<Rightarrow> 'x \<Rightarrow> bool) z x);
-    _ :: unit \<leftarrow> assert_spmf ((A::'y \<Rightarrow> bool) y);
-    return_spmf ((g::'z \<Rightarrow> 'x \<Rightarrow> 'y \<Rightarrow> bool) z x y) }"
-    using bind_commute_spmf by fast
-  then show ?thesis by presburger
+    define ck where ck_def: "ck = map (\<lambda>t. \<^bold>g\<^bsub>G\<^sub>p\<^esub> ^\<^bsub>G\<^sub>p\<^esub> (\<alpha>^t)) [0..<max_deg+1]"
+  define vk where vk_def: "vk = map (\<lambda>t. \<^bold>g\<^bsub>G\<^sub>p\<^esub> ^\<^bsub>G\<^sub>p\<^esub> (\<alpha>^t)) [0..<max_deg+1]"
+  define p_i  where p_i_def: "p_i = fst (Eval ck td (Poly (map (of_int_mod_ring::int \<Rightarrow>'e mod_ring) cvec)) i )" 
+  define w_i  where w_i_def: "w_i = snd (Eval ck td (Poly (map (of_int_mod_ring::int \<Rightarrow>'e mod_ring) cvec)) i )" 
+
+  have "length ck = length cvec 
+        \<and> c = fold (\<lambda> i acc. acc \<otimes> ck!i [^] (cvec!i)) [0..<length ck] \<one> 
+        \<and> verify_eval_batch vk c I (r_x,w) \<and> poly r_x i \<noteq> p_i 
+        \<and> valid_argument_batch I \<and> valid_eval_batch (r_x,w) \<and> i \<in> I 
+        \<longrightarrow>
+          length ck = length cvec 
+        \<and> c = fold (\<lambda> i acc. acc \<otimes> ck!i [^] (cvec!i)) [0..<length ck] \<one> 
+        \<and> i \<in> I \<and> p_i \<noteq> poly r_x i 
+        \<and> valid_argument_batch I \<and> valid_eval (p_i, w_i) \<and> valid_eval_batch (r_x, w) 
+        \<and> verify_eval vk c i (p_i, w_i)
+        \<and> verify_eval_batch vk c I (r_x,w)"
+  (is "?lhs \<longrightarrow> ?rhs")
+  proof 
+    assume asm: "?lhs"
+    show "?rhs"
+    proof(intro conjI)
+      from asm show "length ck = length cvec" by blast
+      from asm show "c = fold (\<lambda>(i::nat) acc::'a. acc \<otimes> ck ! i [^] cvec ! i) [0..<length ck] \<one>" by blast
+      from asm show "i \<in> I" by blast
+      from asm show " p_i \<noteq> poly r_x i" by blast
+      from asm show "valid_argument_batch I" by blast
+      from asm show "valid_eval_batch (r_x, w)" by blast
+      from asm show "verify_eval_batch vk c I (r_x, w)" by blast
+      show "valid_eval (p_i, w_i)" 
+      proof -
+        have "g_pow_PK_Prod ck (\<psi>_of (Poly (map of_int_mod_ring cvec)) i) 
+        = \<^bold>g\<^bsub>G\<^sub>p\<^esub> ^\<^bsub>G\<^sub>p\<^esub> (poly (\<psi>_of (Poly (map of_int_mod_ring cvec)) i) \<alpha>)"
+          unfolding ck_def
+        proof (rule g_pow_PK_Prod_correct)
+          show "degree (\<psi>_of (Poly (map of_int_mod_ring cvec)) i) \<le> max_deg"
+          proof (rule  le_trans[OF degree_q_le_\<phi>])
+            have "length (map of_int_mod_ring cvec) = max_deg +1"
+              using asm unfolding ck_def by force
+            moreover have "length (coeffs (Poly (map of_int_mod_ring cvec))) \<le> length (map of_int_mod_ring cvec)"
+              by (metis coeffs_Poly length_map length_strip_while_le)
+            ultimately show "degree (Poly (map of_int_mod_ring cvec)) \<le> max_deg"
+              using degree_eq_length_coeffs[of "Poly (map of_int_mod_ring cvec)"]
+              by (metis le_diff_conv)
+          qed
+        qed
+        then show ?thesis 
+          unfolding valid_eval_def
+          by (simp add: Eval_def p_i_def w_i_def)
+      qed
+      show "verify_eval vk c i (p_i, w_i)" 
+      proof -
+        let ?cvec = "(map of_int_mod_ring cvec::'e mod_ring list)"
+  
+        have length_cvec: "length ?cvec = max_deg +1"
+          using asm unfolding ck_def by force
+        moreover have "length (coeffs (Poly ?cvec)) \<le> length ?cvec"
+          by (metis coeffs_Poly length_strip_while_le)
+        ultimately have deg_poly_calc_vec_le_max_deg: "degree (Poly ?cvec) \<le> max_deg"
+          using degree_eq_length_coeffs[of "Poly ?cvec"]
+          by (metis coeffs_Poly le_diff_conv length_strip_while_le)
+        
+        have 1: "(g_pow_PK_Prod (map (\<lambda>t. \<^bold>g ^\<^bsub>G\<^sub>p\<^esub> \<alpha> ^ t) [0..<max_deg + 1])
+          (\<psi>_of (Poly ?cvec) i))
+          = (\<^bold>g ^\<^bsub>G\<^sub>p\<^esub> poly (\<psi>_of (Poly ?cvec) i) \<alpha>)"
+        proof(rule  g_pow_PK_Prod_correct)
+          show "degree (\<psi>_of (Poly ?cvec) i) \<le> max_deg"
+            by (rule le_trans[OF degree_q_le_\<phi>])(fact deg_poly_calc_vec_le_max_deg)
+        qed
+  
+        have 2: "map (\<lambda>t. \<^bold>g ^\<^bsub>G\<^sub>p\<^esub> \<alpha> ^ t) [0..<max_deg + 1] ! 1 = \<^bold>g ^\<^bsub>G\<^sub>p\<^esub> \<alpha>"
+          by (metis (no_types, lifting) One_nat_def add.commute d_pos diff_zero le_add_same_cancel1 le_zero_eq length_upt nth_map nth_upt plus_1_eq_Suc power_one_right zero_compare_simps(1))
+        
+        have 3: "(\<^bold>g ^\<^bsub>G\<^sub>p\<^esub> poly (Poly ?cvec) \<alpha>) = c"
+        proof -
+          have "(\<^bold>g ^\<^bsub>G\<^sub>p\<^esub> poly (Poly ?cvec) \<alpha>) 
+               = g_pow_PK_Prod (map (\<lambda>t. \<^bold>g ^\<^bsub>G\<^sub>p\<^esub> \<alpha> ^ t) [0..<max_deg + 1]) (Poly ?cvec)"
+            by (rule g_pow_PK_Prod_correct[symmetric])(fact deg_poly_calc_vec_le_max_deg)
+          also have g_pow_to_fold: "\<dots> = fold (\<lambda>i acc. acc \<otimes>\<^bsub>G\<^sub>p\<^esub> (\<^bold>g\<^bsub>G\<^sub>p\<^esub> ^\<^bsub>G\<^sub>p\<^esub> (\<alpha>^i)) ^\<^bsub>G\<^sub>p\<^esub> (poly.coeff (Poly ?cvec) i)) 
+            [0..<Suc (degree (Poly ?cvec))] \<one>\<^bsub>G\<^sub>p\<^esub>"
+            by (rule g_pow_PK_Prod_to_fold)(fact deg_poly_calc_vec_le_max_deg)
+          also have "\<dots> 
+          =fold (\<lambda> i acc. acc \<otimes>\<^bsub>G\<^sub>p\<^esub> (\<^bold>g\<^bsub>G\<^sub>p\<^esub> ^\<^bsub>G\<^sub>p\<^esub> (\<alpha>^i)) ^\<^bsub>G\<^sub>p\<^esub> (?cvec!i)) [0..<max_deg+1] \<one>\<^bsub>G\<^sub>p\<^esub>"
+          proof -
+            have "fold (\<lambda>i acc. acc \<otimes> (\<^bold>g ^\<^bsub>G\<^sub>p\<^esub> \<alpha> ^ i) ^\<^bsub>G\<^sub>p\<^esub> ?cvec ! i) [0..<max_deg + 1] \<one>
+                = fold (\<lambda>i acc. acc \<otimes> (\<^bold>g ^\<^bsub>G\<^sub>p\<^esub> \<alpha> ^ i) ^\<^bsub>G\<^sub>p\<^esub> ?cvec ! i) 
+                    ([0..<Suc (degree (Poly ?cvec))] @ [Suc (degree (Poly ?cvec))..<max_deg + 1]) 
+                    \<one>" 
+            proof -
+              have "Suc (degree (Poly ?cvec)) \<le> max_deg +1"
+                by (simp add: deg_poly_calc_vec_le_max_deg)
+              then show ?thesis
+                by (metis (lifting) nat_le_iff_add upt_add_eq_append zero_order(1))
+            qed
+            also have "\<dots> = fold (\<lambda>i acc. acc \<otimes> (\<^bold>g ^\<^bsub>G\<^sub>p\<^esub> \<alpha> ^ i) ^\<^bsub>G\<^sub>p\<^esub> ?cvec ! i) 
+                              [Suc (degree (Poly ?cvec))..<max_deg + 1]
+                              (fold (\<lambda>i acc. acc \<otimes> (\<^bold>g ^\<^bsub>G\<^sub>p\<^esub> \<alpha> ^ i) ^\<^bsub>G\<^sub>p\<^esub> ?cvec ! i) 
+                               [0..<Suc (degree (Poly ?cvec))] \<one>)"
+              by fastforce
+            also have "\<dots> = fold (\<lambda>i acc. acc \<otimes> (\<^bold>g ^\<^bsub>G\<^sub>p\<^esub> \<alpha> ^ i) ^\<^bsub>G\<^sub>p\<^esub> poly.coeff (Poly ?cvec) i) 
+                              [0..<Suc (degree (Poly ?cvec))] 
+                              \<one>"
+            proof -
+              have "fold (\<lambda>i acc. acc \<otimes> (\<^bold>g ^\<^bsub>G\<^sub>p\<^esub> \<alpha> ^ i) ^\<^bsub>G\<^sub>p\<^esub> ?cvec ! i) [0..<Suc (degree (Poly ?cvec))] \<one> 
+                  = fold (\<lambda>i acc. acc \<otimes> (\<^bold>g ^\<^bsub>G\<^sub>p\<^esub> \<alpha> ^ i) ^\<^bsub>G\<^sub>p\<^esub> poly.coeff (Poly ?cvec) i) [0..<Suc (degree (Poly ?cvec))] \<one>" 
+              proof (rule List.fold_cong) 
+                show " \<And>x. x \<in> set [0..<Suc (degree (Poly ?cvec))] \<Longrightarrow>
+                         (\<lambda>acc. acc \<otimes> (\<^bold>g ^\<^bsub>G\<^sub>p\<^esub> \<alpha> ^ x) ^\<^bsub>G\<^sub>p\<^esub> ?cvec ! x) =
+                         (\<lambda>acc. acc \<otimes> (\<^bold>g ^\<^bsub>G\<^sub>p\<^esub> \<alpha> ^ x) ^\<^bsub>G\<^sub>p\<^esub> poly.coeff (Poly ?cvec) x)"
+                proof 
+                  fix x::nat
+                  fix acc::'a
+                  assume asm: "x \<in> set [0..<Suc (degree (Poly ?cvec))]"
+                  then have "?cvec ! x = poly.coeff (Poly ?cvec) x"
+                    by (metis \<open>length ?cvec = max_deg + 1\<close> atLeastLessThan_iff coeff_Poly deg_poly_calc_vec_le_max_deg dual_order.trans less_Suc_eq_le nth_default_nth semiring_norm(174) set_upt)
+                  then show "acc \<otimes> (\<^bold>g ^\<^bsub>G\<^sub>p\<^esub> \<alpha> ^ x) ^\<^bsub>G\<^sub>p\<^esub> ?cvec ! x = acc \<otimes> (\<^bold>g ^\<^bsub>G\<^sub>p\<^esub> \<alpha> ^ x) ^\<^bsub>G\<^sub>p\<^esub> poly.coeff (Poly ?cvec) x "
+                    by presburger
+                qed
+              qed simp+
+              moreover have "\<forall>init \<in> carrier G\<^sub>p. 
+                      fold (\<lambda>i acc. acc \<otimes> (\<^bold>g ^\<^bsub>G\<^sub>p\<^esub> \<alpha> ^ i) ^\<^bsub>G\<^sub>p\<^esub> ?cvec ! i) 
+                        [Suc (degree (Poly ?cvec))..<max_deg + 1] 
+                        init 
+                      = init"
+              proof 
+                fix init ::'a
+                assume init_in_carrier: "init \<in> carrier G\<^sub>p"
+                have "fold (\<lambda>i acc. acc \<otimes> (\<^bold>g ^\<^bsub>G\<^sub>p\<^esub> \<alpha> ^ i) ^\<^bsub>G\<^sub>p\<^esub> ?cvec ! i) 
+                        [Suc (degree (Poly ?cvec))..<max_deg + 1]    
+                        init = fold (\<lambda>i acc. acc \<otimes> \<one>) 
+                        [Suc (degree (Poly ?cvec))..<max_deg + 1] 
+                        init"
+                proof (rule List.fold_cong)
+                  show " \<And>x. x \<in> set [Suc (degree (Poly ?cvec))..<max_deg + 1] \<Longrightarrow>
+                          (\<lambda>acc. acc \<otimes> (\<^bold>g ^\<^bsub>G\<^sub>p\<^esub> \<alpha> ^ x) ^\<^bsub>G\<^sub>p\<^esub> ?cvec ! x) = (\<lambda>acc. acc \<otimes> \<one>)"
+                  proof 
+                    fix x::nat
+                    fix acc ::'a
+                    assume asm: "x \<in> set [Suc (degree (Poly ?cvec))..<max_deg + 1]"
+                    show "acc \<otimes> (\<^bold>g ^\<^bsub>G\<^sub>p\<^esub> \<alpha> ^ x) ^\<^bsub>G\<^sub>p\<^esub> ?cvec ! x = acc  \<otimes> \<one>"
+                    proof -
+                      have " ?cvec ! x = 0" using asm length_cvec
+                        by (smt (verit) add.commute coeff_Poly_eq in_set_conv_nth le_degree length_upt less_diff_conv not_less_eq_eq nth_default_eq_dflt_iff nth_upt order.refl trans_le_add2)
+                      then have "(\<^bold>g ^\<^bsub>G\<^sub>p\<^esub> \<alpha> ^ x) ^\<^bsub>G\<^sub>p\<^esub> ?cvec ! x = \<one>" by simp
+                      then show ?thesis by argo 
+                    qed
+                  qed
+                qed simp+
+                also have "\<dots> = init" 
+                proof (induction max_deg)
+                  case 0
+                  then show ?case by fastforce
+                next
+                  case (Suc max_deg)
+                  have "fold (\<lambda>i acc. acc \<otimes> \<one>) [Suc (degree (Poly ?cvec))..<Suc max_deg + 1] init
+                  = fold (\<lambda>i acc. acc \<otimes> \<one>) ([Suc (degree (Poly ?cvec))..<max_deg + 1] @ [Suc max_deg]) init"
+                    by (simp add: init_in_carrier)
+                  also have "\<dots> = fold (\<lambda>i acc. acc \<otimes> \<one>) [Suc max_deg] (fold (\<lambda>i acc. acc \<otimes> \<one>) [Suc (degree (Poly ?cvec))..<max_deg + 1] init)"
+                    by force
+                  also have "\<dots> = fold (\<lambda>i acc. acc \<otimes> \<one>) [Suc max_deg] init" using Suc.IH by argo
+                  also have "\<dots> = init \<otimes> \<one>" by force
+                  also have "\<dots> = init" by (simp add: init_in_carrier)
+                  finally show ?case .
+                qed
+                finally show "fold (\<lambda>i acc. acc \<otimes> (\<^bold>g ^\<^bsub>G\<^sub>p\<^esub> \<alpha> ^ i) ^\<^bsub>G\<^sub>p\<^esub> ?cvec ! i) 
+                        [Suc (degree (Poly ?cvec))..<max_deg + 1] 
+                        init 
+                     = init" .
+              qed
+              ultimately show ?thesis
+                by (metis (no_types, lifting) G\<^sub>p.generator_closed G\<^sub>p.int_pow_closed \<open>\<^bold>g ^\<^bsub>G\<^sub>p\<^esub> poly (Poly ?cvec) \<alpha> = g_pow_PK_Prod (map (\<lambda>t. \<^bold>g ^\<^bsub>G\<^sub>p\<^esub> \<alpha> ^ t) [0..<max_deg + 1]) (Poly ?cvec)\<close> g_pow_to_fold)
+            qed
+            finally show ?thesis by presburger
+          qed
+          also have "\<dots> 
+          =fold (\<lambda> i acc. acc \<otimes>\<^bsub>G\<^sub>p\<^esub> (map (\<lambda>t. \<^bold>g\<^bsub>G\<^sub>p\<^esub> ^\<^bsub>G\<^sub>p\<^esub> (\<alpha>^t)) [0..<max_deg+1])!i ^\<^bsub>G\<^sub>p\<^esub> (?cvec!i)) [0..<max_deg+1] \<one>\<^bsub>G\<^sub>p\<^esub>"
+          proof(rule List.fold_cong)
+            show "\<one> = \<one>" by simp
+            show "[0..<max_deg + 1] = [0..<max_deg + 1]" by simp
+            show "\<And>x. x \<in> set [0..<max_deg + 1] \<Longrightarrow>
+             (\<lambda>acc. acc \<otimes> (\<^bold>g ^\<^bsub>G\<^sub>p\<^esub> \<alpha> ^ x) ^\<^bsub>G\<^sub>p\<^esub> ?cvec ! x) =
+             (\<lambda>acc. acc \<otimes> map (\<lambda>t. \<^bold>g ^\<^bsub>G\<^sub>p\<^esub> \<alpha> ^ t) [0..<max_deg + 1] ! x ^\<^bsub>G\<^sub>p\<^esub> ?cvec ! x)"
+            proof 
+              fix x::nat 
+              fix acc :: 'a
+              assume asm: "x \<in> set [0..<max_deg + 1]"
+              show " acc \<otimes> (\<^bold>g ^\<^bsub>G\<^sub>p\<^esub> \<alpha> ^ x) ^\<^bsub>G\<^sub>p\<^esub> ?cvec ! x 
+                   = acc \<otimes> map (\<lambda>t. \<^bold>g ^\<^bsub>G\<^sub>p\<^esub> \<alpha> ^ t) [0..<max_deg + 1] ! x ^\<^bsub>G\<^sub>p\<^esub> ?cvec ! x"
+                using PK_i[symmetric] asm
+                by (metis Suc_eq_plus1 atLeastLessThan_iff less_Suc_eq_le set_upt)
+            qed
+          qed
+          also have "\<dots> 
+          =fold (\<lambda> i acc. acc \<otimes>\<^bsub>G\<^sub>p\<^esub> (map (\<lambda>t. \<^bold>g\<^bsub>G\<^sub>p\<^esub> ^\<^bsub>G\<^sub>p\<^esub> (\<alpha>^t)) [0..<max_deg+1])!i ^\<^bsub>G\<^sub>p\<^esub> (of_int_mod_ring (cvec!i))) [0..<max_deg+1] \<one>\<^bsub>G\<^sub>p\<^esub>"
+          proof(rule List.fold_cong)
+            fix x
+            assume "x \<in> set [0..<max_deg + 1]"
+            then have "x < length cvec" 
+              using asm unfolding ck_def 
+              by fastforce
+            then show "(\<lambda>acc. acc \<otimes> map (\<lambda>t. \<^bold>g ^ \<alpha> ^ t) [0..<max_deg + 1] ! x ^ map of_int_mod_ring cvec ! x) =
+           (\<lambda>acc. acc \<otimes> map (\<lambda>t. \<^bold>g ^ \<alpha> ^ t) [0..<max_deg + 1] ! x ^ of_int_mod_ring (cvec ! x))"
+              by force
+          qed simp+
+          also have "\<dots> = fold (\<lambda> i acc. acc \<otimes> ck!i [^] (cvec!i)) [0..<length ck] \<one>"
+          proof -
+            have length_eq_max_deg: "length (map (\<lambda>t. \<^bold>g ^ \<alpha> ^ t) [0..<max_deg + 1]) = max_deg +1"
+              by force
+            have mod_ring_trnsf_eq_plain: "\<And>g x. g \<in> carrier G\<^sub>p \<Longrightarrow>  g [^]\<^bsub>G\<^sub>p\<^esub> (to_int_mod_ring (of_int_mod_ring x::'e mod_ring)) = g [^]\<^bsub>G\<^sub>p\<^esub> x"
+            proof -
+              fix g x
+              assume g_in_carrier: "g \<in> carrier G\<^sub>p"
+              have mod_red: "to_int_mod_ring (of_int_mod_ring x::'e mod_ring) = x mod p"
+                unfolding of_int_mod_ring_def to_int_mod_ring_def 
+                by (metis CARD_q of_int_mod_ring.rep_eq of_int_mod_ring_def to_int_mod_ring.rep_eq to_int_mod_ring_def)
+              then show  "g [^]\<^bsub>G\<^sub>p\<^esub> (to_int_mod_ring (of_int_mod_ring x::'e mod_ring)) = g [^]\<^bsub>G\<^sub>p\<^esub> x"
+                using carrier_pow_mod_order_G\<^sub>p g_in_carrier mod_red by metis
+            qed
+            show ?thesis 
+            proof(rule List.fold_cong)
+              fix x 
+              assume "x \<in> set [0..<max_deg + 1]"
+              then show "(\<lambda>acc. acc \<otimes> map (\<lambda>t. \<^bold>g ^ \<alpha> ^ t) [0..<max_deg + 1] ! x ^ of_int_mod_ring (cvec ! x)) = (\<lambda>acc. acc \<otimes> ck ! x [^] cvec ! x)"
+                unfolding ck_def length_eq_max_deg using mod_ring_trnsf_eq_plain 
+                by (metis (no_types, lifting) G\<^sub>p.generator_closed G\<^sub>p.int_pow_closed atLeastLessThan_iff length_upt nth_map set_upt verit_minus_simplify(2))
+            qed (simp add: ck_def)+
+          qed
+          also have "\<dots> = c" 
+            using asm unfolding ck_def by fast
+          finally show ?thesis . 
+        qed
+        show ?thesis
+          unfolding verify_eval_def Eval_def Let_def split_def g_pow_PK_Prod_correct 
+          using eq_on_e[of "(Poly ?cvec)" i \<alpha>]
+          by (metis "1" "2" 3 Eval_def ck_def vk_def p_i_def w_i_def eq_on_e fst_conv snd_conv)
+      qed
+    qed
+  qed
+  then show ?thesis 
+    unfolding ck_def vk_def p_i_def w_i_def Let_def split_def
+    by blast
 qed
 
-lemma pull_down_assert_spmf_with_assert:
-"do {
-    z::'z \<leftarrow> Z:: 'z spmf;
-    x::'x \<leftarrow> (X:: 'z \<Rightarrow> 'x spmf) z;
-    _ :: unit \<leftarrow> assert_spmf((f::'z \<Rightarrow> 'x \<Rightarrow> bool) z x);
-    y::'y \<leftarrow> (Y:: 'z \<Rightarrow> 'x \<Rightarrow> 'y spmf) z x;
-    _ :: unit \<leftarrow> assert_spmf((g::'z \<Rightarrow> 'x \<Rightarrow> 'y \<Rightarrow> bool) z x y);
-    return_spmf True }
-  = do {
-    z::'z \<leftarrow> Z:: 'z spmf;
-    x::'x \<leftarrow> (X:: 'z \<Rightarrow> 'x spmf) z;
-    y::'y \<leftarrow> (Y:: 'z \<Rightarrow> 'x \<Rightarrow> 'y spmf) z x;
-    _ :: unit \<leftarrow> assert_spmf((f::'z \<Rightarrow> 'x \<Rightarrow> bool) z x);
-    _ :: unit \<leftarrow> assert_spmf((g::'z \<Rightarrow> 'x \<Rightarrow> 'y \<Rightarrow> bool) z x y);
-    return_spmf True }"
-proof -
-  have "\<forall>z x. do {
-    _ :: unit \<leftarrow> assert_spmf((f::'z \<Rightarrow> 'x \<Rightarrow> bool) z x);
-    y::'y \<leftarrow> (Y:: 'z \<Rightarrow> 'x \<Rightarrow> 'y spmf) z x;
-    _ :: unit \<leftarrow> assert_spmf((g::'z \<Rightarrow> 'x \<Rightarrow> 'y \<Rightarrow> bool) z x y);
-    return_spmf True }
-  = do {
-    y::'y \<leftarrow> (Y:: 'z \<Rightarrow> 'x \<Rightarrow> 'y spmf) z x;
-    _ :: unit \<leftarrow> assert_spmf((f::'z \<Rightarrow> 'x \<Rightarrow> bool) z x);
-    _ :: unit \<leftarrow> assert_spmf((g::'z \<Rightarrow> 'x \<Rightarrow> 'y \<Rightarrow> bool) z x y);
-    return_spmf True}"
-    using bind_commute_spmf by fast
-  then show ?thesis by presburger
-qed
 
-
-subsection \<open>Reduction proof\<close>
-
-text \<open>We structure the proof in 5 parts:
-
-1. We restate the knowledge soundness game such that all assert statements are combined in one.
-
-2. We restate the evaluation binding game with the extended reduction adversary such that all 
-assert statements are combined in one.
-
-3. We show that the accumulated assert statements in the last two steps are equivalent. Furthermore, 
-we can conclude that the games are in fact equivalent.
-
-4. We conclude from step 1 to 3 that the knowledge soundness game is the same game as the evalutaion 
-binding game for the extended adversary
-
-5. We overestimate the extended reduction with the normal reduction.
-
-6. We conclude from step 4 that the probability of winning the knowledge soundness game is less 
-than or equal to winning the evaluation binding game with the normal reduction adversary. 
-Furthermore, we can conclude transitively through the evaluation binding game, that the probability 
-of the adversary winning the knowledge soundness game is less than or equal to breaking the 
-t-BSDH assumption.
-\<close>
-
-
-text \<open>Proof Step 1:\<close>
-lemma knowledge_soundness_game_alt_def: 
-  "knowledge_soundness_game E \<A> \<A>' = 
-   TRY do {
-    x :: nat \<leftarrow> sample_uniform (order G\<^sub>p);
-    let \<alpha> = of_int_mod_ring (int x);
-    let PK = map (\<lambda>t. \<^bold>g\<^bsub>G\<^sub>p\<^esub> ^\<^bsub>G\<^sub>p\<^esub> (\<alpha>^t)) [0..<max_deg+1];
-    (C,calc_vec, \<sigma>) \<leftarrow> \<A> PK;
-    let \<phi> = E C calc_vec;
-    (i, B, r_x, w_B) \<leftarrow> \<A>' \<sigma> PK C calc_vec;
-    _ :: unit \<leftarrow> assert_spmf (length PK = length calc_vec 
-            \<and> C = fold (\<lambda> i acc. acc \<otimes>\<^bsub>G\<^sub>p\<^esub> PK!i ^\<^bsub>G\<^sub>p\<^esub> (calc_vec!i)) [0..<length PK] \<one>\<^bsub>G\<^sub>p\<^esub>
-            \<and> i \<in> B  
-            \<and> valid_batch_msg r_x w_B B
-            \<and> VerifyEvalBatch PK C B r_x w_B 
-            \<and> poly r_x i \<noteq> poly \<phi> i);
-   return_spmf True
-  } ELSE return_spmf False"
+theorem ks_game_to_eval_bind_game: "spmf (knowledge_soundness_game_AGM \<A>1 \<A>2 E) True 
+  \<le> spmf (bind_game (ks_to_eval_bind_reduction \<A>1 \<A>2 E)) True"
+  (is "?lhs \<le> ?rhs")
 proof -
   note [simp] = Let_def split_def
 
-  text \<open>we rearrange the asserts together in the knowledge soundness game so that we can combine 
-  them later on.\<close>
-  have "do {
-  PK \<leftarrow> KeyGen;
-  (C,calc_vec, \<sigma>) \<leftarrow> \<A> PK;
-  _ :: unit \<leftarrow> assert_spmf (length PK = length calc_vec 
-                          \<and> C = fold (\<lambda> i acc. acc \<otimes>\<^bsub>G\<^sub>p\<^esub> PK!i ^\<^bsub>G\<^sub>p\<^esub> (calc_vec!i)) [0..<length PK] \<one>\<^bsub>G\<^sub>p\<^esub>);  
-  (i, B, r_x, w_B) \<leftarrow> \<A>' \<sigma> PK C calc_vec;
-    _ :: unit \<leftarrow> assert_spmf (i \<in> B  \<and> valid_batch_msg r_x w_B B);
-  return_spmf (VerifyEvalBatch PK C B r_x w_B \<and> poly r_x i \<noteq> poly (E C calc_vec) i)} 
-  = 
-  do {
-  PK \<leftarrow> KeyGen;
-  (C,calc_vec, \<sigma>) \<leftarrow> \<A> PK;
-  (i, B, r_x, w_B) \<leftarrow> \<A>' \<sigma> PK C calc_vec;
-  _ :: unit \<leftarrow> assert_spmf (length PK = length calc_vec 
-                          \<and> C = fold (\<lambda> i acc. acc \<otimes>\<^bsub>G\<^sub>p\<^esub> PK!i ^\<^bsub>G\<^sub>p\<^esub> (calc_vec!i)) [0..<length PK] \<one>\<^bsub>G\<^sub>p\<^esub>);  
-  _ :: unit \<leftarrow> assert_spmf (i \<in> B  \<and> valid_batch_msg r_x w_B B);  
-  return_spmf (VerifyEvalBatch PK C B r_x w_B \<and> poly r_x i \<noteq> poly (E C calc_vec) i)}"
-    using pull_down_assert_spmf_with_return[of KeyGen \<A>] by fastforce
-  then have "knowledge_soundness_game E \<A> \<A>' = 
-  TRY do {
-    PK \<leftarrow> KeyGen;
-    (C,calc_vec, \<sigma>) \<leftarrow> \<A> PK;
-    let \<phi> = E C calc_vec;
-    (i, B, r_x, w_B) \<leftarrow> \<A>' \<sigma> PK C calc_vec;
-    _ :: unit \<leftarrow> assert_spmf (length PK = length calc_vec 
-                            \<and> C = fold (\<lambda> i acc. acc \<otimes>\<^bsub>G\<^sub>p\<^esub> PK!i ^\<^bsub>G\<^sub>p\<^esub> (calc_vec!i)) [0..<length PK] \<one>\<^bsub>G\<^sub>p\<^esub>);  
-    _ :: unit \<leftarrow> assert_spmf (i \<in> B  \<and> valid_batch_msg r_x w_B B);
-    return_spmf (VerifyEvalBatch PK C B r_x w_B \<and> poly r_x i \<noteq> poly (E C calc_vec) i)
-  } ELSE return_spmf False"
-    unfolding knowledge_soundness_game_def by algebra
-  text \<open>Now we unfold the knowledge soundness game to merge multiple asserts together.\<close>
-  also have "\<dots> = TRY do {
-    PK \<leftarrow> KeyGen;
-    TRY do {
-    (C,calc_vec, \<sigma>) \<leftarrow> \<A> PK;
-    TRY do {
-    let \<phi> = E C calc_vec;
-    TRY do {
-    (i, B, r_x, w_B) \<leftarrow> \<A>' \<sigma> PK C calc_vec;
-    TRY do {
-     _ :: unit \<leftarrow> assert_spmf (length PK = length calc_vec 
-                            \<and> C = fold (\<lambda> i acc. acc \<otimes>\<^bsub>G\<^sub>p\<^esub> PK!i ^\<^bsub>G\<^sub>p\<^esub> (calc_vec!i)) [0..<length PK] \<one>\<^bsub>G\<^sub>p\<^esub>);  
-    TRY do {
-    _ :: unit \<leftarrow> assert_spmf (i \<in> B  \<and> valid_batch_msg r_x w_B B);  
-    TRY return_spmf (VerifyEvalBatch PK C B r_x w_B \<and> poly r_x i \<noteq> poly \<phi> i)  ELSE return_spmf False
-    } ELSE return_spmf False
-    } ELSE return_spmf False
-    } ELSE return_spmf False
-    } ELSE return_spmf False
-    } ELSE return_spmf False
-  } ELSE return_spmf False"
-   unfolding split_def Let_def
-   by (fold try_bind_spmf_lossless2[OF lossless_return_spmf])simp
-  text \<open>However, before merging we turn the return statement into another assert\<close>
-  also have "\<dots> = TRY do {
-    PK \<leftarrow> KeyGen;
-    TRY do {
-    (C,calc_vec, \<sigma>) \<leftarrow> \<A> PK;
-    TRY do {
-    let \<phi> = E C calc_vec;
-    TRY do {
-    (i, B, r_x, w_B) \<leftarrow> \<A>' \<sigma> PK C calc_vec;
-    TRY do {
-     _ :: unit \<leftarrow> assert_spmf (length PK = length calc_vec 
-                            \<and> C = fold (\<lambda> i acc. acc \<otimes>\<^bsub>G\<^sub>p\<^esub> PK!i ^\<^bsub>G\<^sub>p\<^esub> (calc_vec!i)) [0..<length PK] \<one>\<^bsub>G\<^sub>p\<^esub>);  
-    TRY do {
-    _ :: unit \<leftarrow> assert_spmf (i \<in> B  \<and> valid_batch_msg r_x w_B B);  
-    _ :: unit \<leftarrow> assert_spmf (VerifyEvalBatch PK C B r_x w_B \<and> poly r_x i \<noteq> poly \<phi> i);
-    return_spmf True
-    } ELSE return_spmf False
-    } ELSE return_spmf False
-    } ELSE return_spmf False
-    } ELSE return_spmf False
-    } ELSE return_spmf False
-  } ELSE return_spmf False"
-    by(auto simp add: try_bind_assert_spmf try_spmf_return_spmf1 intro!: try_spmf_cong bind_spmf_cong)
-  text \<open>Now we add the first two asserts together\<close>
-  also have "\<dots> = TRY do {
-    PK \<leftarrow> KeyGen;
-    TRY do {
-    (C,calc_vec, \<sigma>) \<leftarrow> \<A> PK;
-    TRY do {
-    let \<phi> = E C calc_vec;
-    TRY do {
-    (i, B, r_x, w_B) \<leftarrow> \<A>' \<sigma> PK C calc_vec;
-    TRY do {
-     _ :: unit \<leftarrow> assert_spmf (length PK = length calc_vec 
-            \<and> C = fold (\<lambda> i acc. acc \<otimes>\<^bsub>G\<^sub>p\<^esub> PK!i ^\<^bsub>G\<^sub>p\<^esub> (calc_vec!i)) [0..<length PK] \<one>\<^bsub>G\<^sub>p\<^esub>);  
-    TRY do {
-    _ :: unit \<leftarrow> assert_spmf (i \<in> B  \<and> valid_batch_msg r_x w_B B
-            \<and> VerifyEvalBatch PK C B r_x w_B \<and> poly r_x i \<noteq> poly \<phi> i);
-    return_spmf True
-    } ELSE return_spmf False
-    } ELSE return_spmf False
-    } ELSE return_spmf False
-    } ELSE return_spmf False
-    } ELSE return_spmf False
-  } ELSE return_spmf False"
-    using assert_anding by presburger
-  text \<open>we fold again to merge the remaining asserts\<close>
-   also have "\<dots> = TRY do {
-    PK \<leftarrow> KeyGen;
-    TRY do {
-    (C,calc_vec, \<sigma>) \<leftarrow> \<A> PK;
-    TRY do {
-    let \<phi> = E C calc_vec;
-    TRY do {
-    (i, B, r_x, w_B) \<leftarrow> \<A>' \<sigma> PK C calc_vec;
-    TRY do {
-     _ :: unit \<leftarrow> assert_spmf (length PK = length calc_vec 
-            \<and> C = fold (\<lambda> i acc. acc \<otimes>\<^bsub>G\<^sub>p\<^esub> PK!i ^\<^bsub>G\<^sub>p\<^esub> (calc_vec!i)) [0..<length PK] \<one>\<^bsub>G\<^sub>p\<^esub>);
-    _ :: unit \<leftarrow> assert_spmf (i \<in> B  \<and> valid_batch_msg r_x w_B B
-            \<and> VerifyEvalBatch PK C B r_x w_B \<and> poly r_x i \<noteq> poly \<phi> i);
-    return_spmf True
-    } ELSE return_spmf False
-    } ELSE return_spmf False
-    } ELSE return_spmf False
-    } ELSE return_spmf False
-  } ELSE return_spmf False"
-    unfolding split_def Let_def
-    by(fold try_bind_spmf_lossless2[OF lossless_return_spmf]) simp
-  text \<open>Now we can merge the remaining two asserts\<close>
-   also have "\<dots> = TRY do {
-    PK \<leftarrow> KeyGen;
-    TRY do {
-    (C,calc_vec, \<sigma>) \<leftarrow> \<A> PK;
-    TRY do {
-    let \<phi> = E C calc_vec;
-    TRY do {
-    (i, B, r_x, w_B) \<leftarrow> \<A>' \<sigma> PK C calc_vec;
-    TRY do {
-     _ :: unit \<leftarrow> assert_spmf (length PK = length calc_vec 
-            \<and> C = fold (\<lambda> i acc. acc \<otimes>\<^bsub>G\<^sub>p\<^esub> PK!i ^\<^bsub>G\<^sub>p\<^esub> (calc_vec!i)) [0..<length PK] \<one>\<^bsub>G\<^sub>p\<^esub>
-            \<and> i \<in> B  \<and> valid_batch_msg r_x w_B B
-            \<and> VerifyEvalBatch PK C B r_x w_B \<and> poly r_x i \<noteq> poly \<phi> i);
-    return_spmf True
-    } ELSE return_spmf False
-    } ELSE return_spmf False
-    } ELSE return_spmf False
-    } ELSE return_spmf False
-  } ELSE return_spmf False"
-     using assert_anding by presburger
-  text \<open>next we fold the game together to obtain a clean game with all asserts accumulated.\<close>
-  also have "\<dots> = TRY do {
-    PK \<leftarrow> KeyGen;
-    (C,calc_vec, \<sigma>) \<leftarrow> \<A> PK;
-    let \<phi> = E C calc_vec;
-    (i, B, r_x, w_B) \<leftarrow> \<A>' \<sigma> PK C calc_vec;
-     _ :: unit \<leftarrow> assert_spmf (length PK = length calc_vec 
-            \<and> C = fold (\<lambda> i acc. acc \<otimes>\<^bsub>G\<^sub>p\<^esub> PK!i ^\<^bsub>G\<^sub>p\<^esub> (calc_vec!i)) [0..<length PK] \<one>\<^bsub>G\<^sub>p\<^esub>
-            \<and> i \<in> B  \<and> valid_batch_msg r_x w_B B
-            \<and> VerifyEvalBatch PK C B r_x w_B \<and> poly r_x i \<noteq> poly \<phi> i);
-    return_spmf True
-  } ELSE return_spmf False"
-    unfolding split_def Let_def
-    by(fold try_bind_spmf_lossless2[OF lossless_return_spmf]) simp
-  text \<open>Lastly we want to make the construction of PK accessible in the assert. 
-    For that we have to take two steps. Firstly we have unfold KeyGen to obtain access to the 
-    computation of PK.\<close>
-  also have "\<dots> = TRY do {
-    x :: nat \<leftarrow> sample_uniform (order G\<^sub>p);
-    let \<alpha> = of_int_mod_ring (int x);
-    PK \<leftarrow> return_spmf (map (\<lambda>t. \<^bold>g\<^bsub>G\<^sub>p\<^esub> ^\<^bsub>G\<^sub>p\<^esub> (\<alpha>^t)) [0..<max_deg+1]);
-    (C,calc_vec, \<sigma>) \<leftarrow> \<A> PK;
-    let \<phi> = E C calc_vec;
-    (i, B, r_x, w_B) \<leftarrow> \<A>' \<sigma> PK C calc_vec;
-     _ :: unit \<leftarrow> assert_spmf (length PK = length calc_vec 
-            \<and> C = fold (\<lambda> i acc. acc \<otimes>\<^bsub>G\<^sub>p\<^esub> PK!i ^\<^bsub>G\<^sub>p\<^esub> (calc_vec!i)) [0..<length PK] \<one>\<^bsub>G\<^sub>p\<^esub>
-            \<and> i \<in> B  \<and> valid_batch_msg r_x w_B B
-            \<and> VerifyEvalBatch PK C B r_x w_B \<and> poly r_x i \<noteq> poly \<phi> i);
-    return_spmf True
-  } ELSE return_spmf False"
-     using key_gen_alt_def
-     by (smt (verit, ccfv_SIG) bind_spmf_assoc bind_spmf_cong)
-  text \<open>Secondly, we have to unwrap the definition of PK from the spmf into a constant one. 
-   If PK is constant, we can drag its definition into the assert, instead of the variable 
-   PK.\<close>
-    also have "\<dots> = TRY do {
-    x :: nat \<leftarrow> sample_uniform (order G\<^sub>p);
-    let \<alpha> = of_int_mod_ring (int x);
-    let PK = map (\<lambda>t. \<^bold>g\<^bsub>G\<^sub>p\<^esub> ^\<^bsub>G\<^sub>p\<^esub> (\<alpha>^t)) [0..<max_deg+1];
-    (C,calc_vec, \<sigma>) \<leftarrow> \<A> PK;
-    let \<phi> = E C calc_vec;
-    (i, B, r_x, w_B) \<leftarrow> \<A>' \<sigma> PK C calc_vec;
-     _ :: unit \<leftarrow> assert_spmf (length PK = length calc_vec 
-            \<and> C = fold (\<lambda> i acc. acc \<otimes>\<^bsub>G\<^sub>p\<^esub> PK!i ^\<^bsub>G\<^sub>p\<^esub> (calc_vec!i)) [0..<length PK] \<one>\<^bsub>G\<^sub>p\<^esub>
-            \<and> i \<in> B  \<and> valid_batch_msg r_x w_B B
-            \<and> VerifyEvalBatch PK C B r_x w_B \<and> poly r_x i \<noteq> poly \<phi> i);
-    return_spmf True
-  } ELSE return_spmf False"
-      using return_bind_spmf by meson
+  have "spmf (knowledge_soundness_game_AGM \<A>1 \<A>2 E) True = spmf (TRY do {
+      (ck,vk) \<leftarrow> key_gen;
+      ((c,cvec),\<sigma>) \<leftarrow> \<A>1 ck;
+      _ :: unit \<leftarrow> assert_spmf (length ck = length cvec 
+          \<and> c = fold (\<lambda> i acc. acc \<otimes> ck!i [^] (cvec!i)) [0..<length ck] \<one>);
+      (p,td) \<leftarrow> E (c,cvec);
+      (i, I, (r, (w, wvec))) \<leftarrow> AGM2.restrict \<A>2 (ck,\<sigma>);
+      let (p_i,w') = Eval ck td p i;        
+      return_spmf (verify_eval_batch vk c I (r,w) \<and> poly r i \<noteq> p_i 
+        \<and> valid_argument_batch I \<and> valid_eval_batch (r,w) \<and> i \<in> I)       
+    } ELSE return_spmf False) True"
+    unfolding knowledge_soundness_game_AGM_def AGM1.restrict_def listS_def G\<^sub>p.groupS_def noSelect_def 
+        Restrictive_Comp.restrict_def prodC_def G\<^sub>p.groupC_def G\<^sub>p.constrain_grp_def 
+        noConstrain_def
+    by force
+  also have "\<dots>= spmf (TRY do {
+      (ck,vk) \<leftarrow> key_gen;
+      TRY do {
+        ((c,cvec),\<sigma>) \<leftarrow> \<A>1 ck;
+          TRY do {
+          _ :: unit \<leftarrow> assert_spmf (length ck = length cvec 
+              \<and> c = fold (\<lambda> i acc. acc \<otimes> ck!i [^] (cvec!i)) [0..<length ck] \<one>);
+            TRY do {
+            (p,td) \<leftarrow> E (c,cvec);
+              TRY do {
+              (i, I, (r, (w, wvec))) \<leftarrow> AGM2.restrict \<A>2 (ck,\<sigma>);
+              let (p_i,w') = Eval ck td p i;        
+                TRY do {
+                return_spmf (verify_eval_batch vk c I (r,w) \<and> poly r i \<noteq> p_i 
+                  \<and> valid_argument_batch I \<and> valid_eval_batch (r,w) \<and> i \<in> I)    
+              } ELSE return_spmf False   
+            } ELSE return_spmf False
+          } ELSE return_spmf False
+        } ELSE return_spmf False
+      } ELSE return_spmf False
+    } ELSE return_spmf False) True"
+    unfolding Let_def split_def
+    by (fold try_bind_spmf_lossless2[OF lossless_return_spmf])simp
+  also have "\<dots>= spmf (TRY do {
+      (ck,vk) \<leftarrow> key_gen;
+      TRY do {
+        ((c,cvec),\<sigma>) \<leftarrow> \<A>1 ck;
+          TRY do {
+          _ :: unit \<leftarrow> assert_spmf (length ck = length cvec 
+              \<and> c = fold (\<lambda> i acc. acc \<otimes> ck!i [^] (cvec!i)) [0..<length ck] \<one>);
+            TRY do {
+            (p,td) \<leftarrow> E (c,cvec);
+              TRY do {
+              (i, I, (r, (w, wvec))) \<leftarrow> AGM2.restrict \<A>2 (ck,\<sigma>);
+              let (p_i,w') = Eval ck td p i;   
+                TRY do {
+                _ :: unit \<leftarrow> assert_spmf (verify_eval_batch vk c I (r,w) \<and> poly r i \<noteq> p_i 
+                  \<and> valid_argument_batch I \<and> valid_eval_batch (r,w) \<and> i \<in> I);     
+                return_spmf True
+              } ELSE return_spmf False
+            } ELSE return_spmf False
+          } ELSE return_spmf False
+        } ELSE return_spmf False
+      } ELSE return_spmf False
+    } ELSE return_spmf False) True" 
+      by (rule spmf_eqI')(auto simp add:  try_bind_assert_spmf try_spmf_return_spmf1 del: Let_def split_def intro!: try_spmf_cong bind_spmf_cong)
+      also have "\<dots>= spmf (TRY do {
+      (ck,vk) \<leftarrow> key_gen;
+      ((c,cvec),\<sigma>) \<leftarrow> \<A>1 ck;
+      _ :: unit \<leftarrow> assert_spmf (length ck = length cvec 
+       \<and> c = fold (\<lambda> i acc. acc \<otimes> ck!i [^] (cvec!i)) [0..<length ck] \<one>);
+      (p,td) \<leftarrow> E (c,cvec);
+       (i, I, (r, (w, wvec))) \<leftarrow> AGM2.restrict \<A>2 (ck,\<sigma>);
+       let (p_i,w') = Eval ck td p i;
+      _ :: unit \<leftarrow> assert_spmf (verify_eval_batch vk c I (r,w) \<and> poly r i \<noteq> p_i 
+        \<and> valid_argument_batch I \<and> valid_eval_batch (r,w) \<and> i \<in> I);     
+      return_spmf True
+      } ELSE return_spmf False) True"
+        unfolding Let_def split_def
+        by (fold try_bind_spmf_lossless2[OF lossless_return_spmf])simp
+    also have "\<dots>= spmf(TRY do {
+      (ck,vk) \<leftarrow> key_gen;
+      ((c,cvec),\<sigma>) \<leftarrow> \<A>1 ck;
+      (p,td) \<leftarrow> E (c,cvec);
+      (i, I, (r, (w, wvec))) \<leftarrow> AGM2.restrict \<A>2 (ck,\<sigma>);
+      let (p_i,w') = Eval ck td p i;
+      _ :: unit \<leftarrow> assert_spmf (length ck = length cvec 
+       \<and> c = fold (\<lambda> i acc. acc \<otimes> ck!i [^] (cvec!i)) [0..<length ck] \<one>);
+      _ :: unit \<leftarrow> assert_spmf (verify_eval_batch vk c I (r,w) \<and> poly r i \<noteq> p_i 
+        \<and> valid_argument_batch I \<and> valid_eval_batch (r,w) \<and> i \<in> I);     
+      return_spmf True
+      } ELSE return_spmf False) True"
+      apply (rule spmf_eqI')
+      apply (rule try_spmf_cong)
+       apply (rule unpack_bind_spmf'; simp)+
+       apply (subst assert_commute)
+       apply simp+
+      done
+    also have "\<dots>= spmf (TRY do {
+      x :: nat \<leftarrow> sample_uniform (order G\<^sub>p);
+      let (\<alpha>::'e mod_ring) = of_int_mod_ring (int x);
+      let ck = map (\<lambda>t. \<^bold>g\<^bsub>G\<^sub>p\<^esub> ^\<^bsub>G\<^sub>p\<^esub> (\<alpha>^t)) [0..<max_deg+1];
+      let vk = map (\<lambda>t. \<^bold>g\<^bsub>G\<^sub>p\<^esub> ^\<^bsub>G\<^sub>p\<^esub> (\<alpha>^t)) [0..<max_deg+1];
+      ((c,cvec),\<sigma>) \<leftarrow> \<A>1 ck;
+      let (p,td) = (Poly (map (of_int_mod_ring::int \<Rightarrow>'e mod_ring) cvec),());
+      (i, I, (r_x, (w, wvec))) \<leftarrow> AGM2.restrict \<A>2 (ck,\<sigma>);
+      let (p_i,w') = Eval ck td p i;
+      _ :: unit \<leftarrow> assert_spmf (length ck = length cvec 
+        \<and> c = fold (\<lambda> i acc. acc \<otimes> ck!i [^] (cvec!i)) [0..<length ck] \<one> 
+        \<and> verify_eval_batch vk c I (r_x,w) \<and> poly r_x i \<noteq> p_i 
+        \<and> valid_argument_batch I \<and> valid_eval_batch (r_x,w) \<and> i \<in> I);     
+      return_spmf True
+      } ELSE return_spmf False) True"
+      by (simp add: key_gen_def Setup_def assert_collapse)
+    also have "\<dots>\<le> spmf (TRY do {
+      x :: nat \<leftarrow> sample_uniform (order G\<^sub>p);
+      let (\<alpha>::'e mod_ring) = of_int_mod_ring (int x);
+      let ck = map (\<lambda>t. \<^bold>g\<^bsub>G\<^sub>p\<^esub> ^\<^bsub>G\<^sub>p\<^esub> (\<alpha>^t)) [0..<max_deg+1];
+      let vk = map (\<lambda>t. \<^bold>g\<^bsub>G\<^sub>p\<^esub> ^\<^bsub>G\<^sub>p\<^esub> (\<alpha>^t)) [0..<max_deg+1];
+      ((c,cvec),\<sigma>) \<leftarrow> \<A>1 ck;
+      let (p,td) = (Poly (map (of_int_mod_ring::int \<Rightarrow>'e mod_ring) cvec),());
+      (i, I, (r_x, (w, wvec))) \<leftarrow> AGM2.restrict \<A>2 (ck,\<sigma>);
+      let (p_i,w_i) = Eval ck td p i;
+      _ :: unit \<leftarrow> assert_spmf (length ck = length cvec 
+        \<and> c = fold (\<lambda> i acc. acc \<otimes> ck!i [^] (cvec!i)) [0..<length ck] \<one> 
+        \<and> i \<in> I \<and> p_i \<noteq> poly r_x i 
+        \<and> valid_argument_batch I \<and> valid_eval (p_i, w_i) \<and> valid_eval_batch (r_x, w) 
+        \<and> verify_eval vk c i (p_i, w_i)
+        \<and> verify_eval_batch vk c I (r_x,w));     
+      return_spmf True
+      } ELSE return_spmf False) True"
+      unfolding E.simps key_gen_def Setup_def
+      apply (rule try_spmf_le)
+      apply (unfold Let_def split_def)
+      apply (rule bind_spmf_le)+
+      apply (rule assert_imp)
+      apply (insert reduction_map_imp)
+      apply(unfold Let_def split_def)
+      apply (intro impI)
+      apply simp
+      apply force
+      done
+    also have "\<dots>= spmf (TRY do {
+      (ck,vk) \<leftarrow> key_gen;
+      ((c,cvec),\<sigma>) \<leftarrow> \<A>1 ck;
+      (p,td) \<leftarrow> E (c,cvec);
+      (i, I, (r_x, (w, wvec))) \<leftarrow> AGM2.restrict \<A>2 (ck,\<sigma>);
+      let (p_i,w_i) = Eval ck td p i;
+      _ :: unit \<leftarrow> assert_spmf (length ck = length cvec 
+        \<and> c = fold (\<lambda> i acc. acc \<otimes> ck!i [^] (cvec!i)) [0..<length ck] \<one> 
+        \<and> i \<in> I \<and> p_i \<noteq> poly r_x i 
+        \<and> valid_argument_batch I \<and> valid_eval (p_i, w_i) \<and> valid_eval_batch (r_x, w) 
+        \<and> verify_eval vk c i (p_i, w_i)
+        \<and> verify_eval_batch vk c I (r_x,w));     
+      return_spmf True
+      } ELSE return_spmf False) True"
+      by (simp add: key_gen_def Setup_def assert_collapse)
+    also have "\<dots>= spmf (TRY do {
+      (ck,vk) \<leftarrow> key_gen;
+      ((c,cvec),\<sigma>) \<leftarrow> \<A>1 ck;
+      (p,td) \<leftarrow> E (c,cvec);
+      (i, I, (r_x, (w, wvec))) \<leftarrow> AGM2.restrict \<A>2 (ck,\<sigma>);
+      let (p_i,w_i) = Eval ck td p i;
+      _ :: unit \<leftarrow> assert_spmf (length ck = length cvec 
+        \<and> c = fold (\<lambda> i acc. acc \<otimes> ck!i [^] (cvec!i)) [0..<length ck] \<one> 
+        \<and> i \<in> I \<and> p_i \<noteq> poly r_x i 
+        \<and> valid_argument_batch I \<and> valid_eval (p_i, w_i) \<and> valid_eval_batch (r_x, w));
+      _::unit \<leftarrow> assert_spmf (verify_eval vk c i (p_i, w_i)
+        \<and> verify_eval_batch vk c I (r_x,w));     
+      return_spmf True
+      } ELSE return_spmf False) True"
+      by (simp add: assert_collapse)
+    also have "\<dots>= spmf (TRY do {
+      (ck,vk) \<leftarrow> key_gen;
+        TRY do {
+        ((c,cvec),\<sigma>) \<leftarrow> \<A>1 ck;
+          TRY do {
+          (p,td) \<leftarrow> E (c,cvec);
+            TRY do{
+            (i, I, (r_x, (w, wvec))) \<leftarrow> AGM2.restrict \<A>2 (ck,\<sigma>);
+              TRY do{
+              let (p_i,w_i) = Eval ck td p i;
+              _ :: unit \<leftarrow> assert_spmf (length ck = length cvec 
+        \<and> c = fold (\<lambda> i acc. acc \<otimes> ck!i [^] (cvec!i)) [0..<length ck] \<one> 
+        \<and> i \<in> I \<and> p_i \<noteq> poly r_x i 
+                \<and> valid_argument_batch I \<and> valid_eval (p_i, w_i) \<and> valid_eval_batch (r_x, w));
+                TRY do {
+                _::unit \<leftarrow> assert_spmf (verify_eval vk c i (p_i, w_i)
+                  \<and> verify_eval_batch vk c I (r_x,w));     
+                return_spmf True
+                } ELSE return_spmf False
+              } ELSE return_spmf False
+            } ELSE return_spmf False
+          } ELSE return_spmf False
+        } ELSE return_spmf False
+      } ELSE return_spmf False) True"
+      unfolding Let_def split_def
+      by (fold try_bind_spmf_lossless2[OF lossless_return_spmf])simp
+    also have "\<dots>= spmf (TRY do {
+      (ck,vk) \<leftarrow> key_gen;
+        TRY do {
+        ((c,cvec),\<sigma>) \<leftarrow> \<A>1 ck;
+          TRY do {
+          (p,td) \<leftarrow> E (c,cvec);
+            TRY do{
+            (i, I, (r_x, (w, wvec))) \<leftarrow> AGM2.restrict \<A>2 (ck,\<sigma>);
+              TRY do{
+              let (p_i,w_i) = Eval ck td p i;
+              _ :: unit \<leftarrow> assert_spmf (length ck = length cvec 
+                \<and> c = fold (\<lambda> i acc. acc \<otimes> ck!i [^] (cvec!i)) [0..<length ck] \<one> 
+                \<and> i \<in> I \<and> p_i \<noteq> poly r_x i 
+                \<and> valid_argument_batch I \<and> valid_eval (p_i, w_i) \<and> valid_eval_batch (r_x, w));
+                TRY do {
+                return_spmf (verify_eval vk c i (p_i, w_i)
+                  \<and> verify_eval_batch vk c I (r_x,w))
+                } ELSE return_spmf False
+              } ELSE return_spmf False
+            } ELSE return_spmf False
+          } ELSE return_spmf False
+        } ELSE return_spmf False
+      } ELSE return_spmf False) True"
+      by (rule spmf_eqI')(auto simp add:  try_bind_assert_spmf try_spmf_return_spmf1 del: Let_def split_def intro!: try_spmf_cong bind_spmf_cong)
+    also have "\<dots>= spmf (TRY do {
+      (ck,vk) \<leftarrow> key_gen;
+      ((c,cvec),\<sigma>) \<leftarrow> \<A>1 ck;
+      (p,td) \<leftarrow> E (c,cvec);
+      (i, I, (r_x, (w, wvec))) \<leftarrow> AGM2.restrict \<A>2 (ck,\<sigma>);
+      let (p_i,w_i) = Eval ck td p i;
+      _ :: unit \<leftarrow> assert_spmf (length ck = length cvec 
+        \<and> c = fold (\<lambda> i acc. acc \<otimes> ck!i [^] (cvec!i)) [0..<length ck] \<one> 
+        \<and> i \<in> I \<and> p_i \<noteq> poly r_x i 
+        \<and> valid_argument_batch I \<and> valid_eval (p_i, w_i) \<and> valid_eval_batch (r_x, w));
+      return_spmf (verify_eval vk c i (p_i, w_i)
+        \<and> verify_eval_batch vk c I (r_x,w))
+      } ELSE return_spmf False) True"
+    unfolding Let_def split_def
+    by (fold try_bind_spmf_lossless2[OF lossless_return_spmf])simp
+  also have "\<dots>= spmf (TRY do {
+      (ck,vk) \<leftarrow> key_gen;
+      ((c,cvec),\<sigma>) \<leftarrow> \<A>1 ck;
+      (p,td) \<leftarrow> E (c,cvec);
+      (i, I, (r_x, (w, wvec))) \<leftarrow> AGM2.restrict \<A>2 (ck,\<sigma>);
+      let (p_i,w_i) = Eval ck td p i;
+      _ :: unit \<leftarrow> assert_spmf (length ck = length cvec 
+        \<and> c = fold (\<lambda> i acc. acc \<otimes> ck!i [^] (cvec!i)) [0..<length ck] \<one> );
+      _ :: unit \<leftarrow> assert_spmf (i \<in> I \<and> p_i \<noteq> poly r_x i 
+        \<and> valid_argument_batch I \<and> valid_eval (p_i, w_i) \<and> valid_eval_batch (r_x, w));
+      return_spmf (verify_eval vk c i (p_i, w_i)
+        \<and> verify_eval_batch vk c I (r_x,w))
+      } ELSE return_spmf False) True"
+    by (simp add: assert_collapse)
+    also have "\<dots>= spmf (TRY do {
+      (ck,vk) \<leftarrow> key_gen;
+      ((c,cvec),\<sigma>) \<leftarrow> \<A>1 ck;
+      _ :: unit \<leftarrow> assert_spmf (length ck = length cvec 
+        \<and> c = fold (\<lambda> i acc. acc \<otimes> ck!i [^] (cvec!i)) [0..<length ck] \<one> );
+      (p,td) \<leftarrow> E (c,cvec);
+      (i, I, (r_x, (w, wvec))) \<leftarrow> AGM2.restrict \<A>2 (ck,\<sigma>);
+      let (p_i,w_i) = Eval ck td p i;
+      _ :: unit \<leftarrow> assert_spmf (i \<in> I \<and> p_i \<noteq> poly r_x i 
+        \<and> valid_argument_batch I \<and> valid_eval (p_i, w_i) \<and> valid_eval_batch (r_x, w));
+      return_spmf (verify_eval vk c i (p_i, w_i)
+        \<and> verify_eval_batch vk c I (r_x,w))
+      } ELSE return_spmf False) True"
+      apply (rule spmf_eqI')
+      apply (unfold Let_def split_def)
+      apply (simp split: prod.split)
+      apply (rule unpack_try_spmf)
+      apply (rule unpack_bind_spmf'; rule ext)+
+      apply (subst assert_commute)
+      apply (subst assert_commute)
+      apply blast
+      done
+  also have "\<dots> \<le> spmf (bind_game (ks_to_eval_bind_reduction \<A>1 \<A>2 E)) True"
+    unfolding bind_game_def ks_to_eval_bind_reduction_def
+    unfolding knowledge_soundness_game_AGM_def AGM1.restrict_def listS_def G\<^sub>p.groupS_def noSelect_def 
+        Restrictive_Comp.restrict_def prodC_def G\<^sub>p.groupC_def G\<^sub>p.constrain_grp_def 
+        noConstrain_def split_def Let_def
+    by force
   finally show ?thesis .
 qed
 
-text \<open>Proof Step 2:\<close>
-lemma bind_game_knowledge_soundness_reduction_alt_def: 
-  "bind_game (knowledge_soundness_reduction_ext E \<A> \<A>') = 
-  TRY do {
-    x :: nat \<leftarrow> sample_uniform (order G\<^sub>p);
-    let \<alpha> = of_int_mod_ring (int x);
-    let PK = map (\<lambda>t. \<^bold>g\<^bsub>G\<^sub>p\<^esub> ^\<^bsub>G\<^sub>p\<^esub> (\<alpha>^t)) [0..<max_deg+1];
-    (C,calc_vec, \<sigma>) \<leftarrow> \<A> PK;
-    let \<phi> = E C calc_vec;
-    (i, B, r_x, w_B) \<leftarrow> \<A>' \<sigma> PK C calc_vec;
-    _ :: unit \<leftarrow> assert_spmf (length PK = length calc_vec
-            \<and> C = fold (\<lambda> i acc. acc \<otimes>\<^bsub>G\<^sub>p\<^esub> PK!i ^\<^bsub>G\<^sub>p\<^esub> (calc_vec!i)) [0..<length PK] \<one>\<^bsub>G\<^sub>p\<^esub>
-            \<and> i \<in> B 
-            \<and> poly \<phi> i \<noteq>  poly r_x i
-            \<and> valid_msg (poly \<phi> i) (createWitness PK \<phi> i)
-            \<and> valid_batch_msg r_x w_B B
-            \<and> VerifyEval PK C i (poly \<phi> i) (createWitness PK \<phi> i) 
-            \<and> VerifyEvalBatch PK C B r_x w_B);
-       return_spmf True
-    } ELSE return_spmf False"
-proof -
-  text \<open>Firstly we extract the return value from the evaluation binding game into a assert statement.\<close>
-  have "bind_game (knowledge_soundness_reduction_ext E \<A> \<A>') = TRY do {
-  PK \<leftarrow> KeyGen;
-  (C, i, \<phi>_i, w_i, B, w_B, r_x) \<leftarrow> (knowledge_soundness_reduction_ext E \<A> \<A>') PK;
-  _ :: unit \<leftarrow> assert_spmf (i \<in> B \<and> \<phi>_i \<noteq> poly r_x i \<and> valid_msg \<phi>_i w_i \<and> valid_batch_msg r_x w_B B); 
-  let b = VerifyEval PK C i \<phi>_i w_i;
-  let b' = VerifyEvalBatch PK C B r_x w_B;
-  _::unit \<leftarrow> assert_spmf (b \<and> b');
-  return_spmf True} ELSE return_spmf False" 
-    by (fact bind_game_alt_def)
-  text \<open>Secondly, we inline the extended knowledge soundness adversary, so we can accumulate
-  the asserts from the reduction and the game together.\<close>
-  also have "\<dots> = TRY do {
-  PK \<leftarrow> KeyGen;
-  (C,calc_vec, \<sigma>) \<leftarrow> \<A> PK;
-  _ :: unit \<leftarrow> assert_spmf (length PK = length calc_vec 
-                          \<and> C = fold (\<lambda> i acc. acc \<otimes>\<^bsub>G\<^sub>p\<^esub> PK!i ^\<^bsub>G\<^sub>p\<^esub> (calc_vec!i)) [0..<length PK] \<one>\<^bsub>G\<^sub>p\<^esub>);  
-  let \<phi> = E C calc_vec;
-  (i, B, r_x, w_B) \<leftarrow> \<A>' \<sigma> PK C calc_vec;
-  let \<phi>_i = poly \<phi> i;
-  let w_i = createWitness PK \<phi> i;
-  _ :: unit \<leftarrow> assert_spmf (i \<in> B \<and> \<phi>_i \<noteq> poly r_x i \<and> valid_msg \<phi>_i w_i \<and> valid_batch_msg r_x w_B B); 
-  let b = VerifyEval PK C i \<phi>_i w_i;
-  let b' = VerifyEvalBatch PK C B r_x w_B;
-  _::unit \<leftarrow> assert_spmf (b \<and> b');
-  return_spmf True} ELSE return_spmf False"
-    unfolding knowledge_soundness_reduction_ext_def by (simp add: split_def Let_def)
-  text \<open>We fold the game into smaller sub games, such that we can combine the individual asserts.\<close>
-  also have "\<dots> = TRY do {
-    PK \<leftarrow> KeyGen;
-    TRY do{
-    (C,calc_vec, \<sigma>) \<leftarrow> \<A> PK;
-    TRY do {
-    _ :: unit \<leftarrow> assert_spmf (length PK = length calc_vec 
-                            \<and> C = fold (\<lambda> i acc. acc \<otimes>\<^bsub>G\<^sub>p\<^esub> PK!i ^\<^bsub>G\<^sub>p\<^esub> (calc_vec!i)) [0..<length PK] \<one>\<^bsub>G\<^sub>p\<^esub>);  
-    let \<phi> = E C calc_vec;
-    TRY do {
-    (i, B, r_x, w_B) \<leftarrow> \<A>' \<sigma> PK C calc_vec;
-    let \<phi>_i = poly \<phi> i;
-    let w_i = createWitness PK \<phi> i;
-    TRY do {
-    _ :: unit \<leftarrow> assert_spmf (i \<in> B \<and> \<phi>_i \<noteq> poly r_x i \<and> valid_msg \<phi>_i w_i \<and> valid_batch_msg r_x w_B B); 
-    let b = VerifyEval PK C i \<phi>_i w_i;
-    let b' = VerifyEvalBatch PK C B r_x w_B;
-    _::unit \<leftarrow> assert_spmf (b \<and> b');
-    return_spmf True
-    } ELSE return_spmf False 
-    } ELSE return_spmf False 
-    } ELSE return_spmf False 
-    } ELSE return_spmf False 
-  } ELSE return_spmf False"
-   unfolding split_def Let_def 
-   by(fold try_bind_spmf_lossless2[OF lossless_return_spmf]) simp
-  text \<open>We combine the first two asserts\<close>
-  also have "\<dots> = TRY do {
-    PK \<leftarrow> KeyGen;
-    TRY do{
-    (C,calc_vec, \<sigma>) \<leftarrow> \<A> PK;
-    TRY do {
-    _ :: unit \<leftarrow> assert_spmf (length PK = length calc_vec 
-                            \<and> C = fold (\<lambda> i acc. acc \<otimes>\<^bsub>G\<^sub>p\<^esub> PK!i ^\<^bsub>G\<^sub>p\<^esub> (calc_vec!i)) [0..<length PK] \<one>\<^bsub>G\<^sub>p\<^esub>);  
-    let \<phi> = E C calc_vec;
-    TRY do {
-    (i, B, r_x, w_B) \<leftarrow> \<A>' \<sigma> PK C calc_vec;
-    let \<phi>_i = poly \<phi> i;
-    let w_i = createWitness PK \<phi> i;
-    TRY do {
-    _ :: unit \<leftarrow> assert_spmf (i \<in> B \<and> \<phi>_i \<noteq> poly r_x i 
-                            \<and> valid_msg \<phi>_i w_i \<and> valid_batch_msg r_x w_B B
-                            \<and> VerifyEval PK C i \<phi>_i w_i \<and> VerifyEvalBatch PK C B r_x w_B);
-    return_spmf True
-    } ELSE return_spmf False 
-    } ELSE return_spmf False 
-    } ELSE return_spmf False 
-    } ELSE return_spmf False 
-  } ELSE return_spmf False"
-    using assert_anding by presburger
-  text \<open>We fold the game into one coherent game again to rearrange asserts.
-  We aim to bring the asserts closer together so we can merge them.\<close> 
-  also have "\<dots> = TRY do {
-    PK \<leftarrow> KeyGen;
-    (C,calc_vec, \<sigma>) \<leftarrow> \<A> PK;
-    _ :: unit \<leftarrow> assert_spmf (length PK = length calc_vec 
-                            \<and> C = fold (\<lambda> i acc. acc \<otimes>\<^bsub>G\<^sub>p\<^esub> PK!i ^\<^bsub>G\<^sub>p\<^esub> (calc_vec!i)) [0..<length PK] \<one>\<^bsub>G\<^sub>p\<^esub>);  
-    let \<phi> = E C calc_vec;
-    (i, B, r_x, w_B) \<leftarrow> \<A>' \<sigma> PK C calc_vec;
-    let \<phi>_i = poly \<phi> i;
-    let w_i = createWitness PK \<phi> i;
-    _ :: unit \<leftarrow> assert_spmf (i \<in> B \<and> \<phi>_i \<noteq> poly r_x i 
-                            \<and> valid_msg \<phi>_i w_i \<and> valid_batch_msg r_x w_B B
-                            \<and> VerifyEval PK C i \<phi>_i w_i \<and> VerifyEvalBatch PK C B r_x w_B);
-    return_spmf True
-  } ELSE return_spmf False"
-   unfolding split_def Let_def 
-   by(fold try_bind_spmf_lossless2[OF lossless_return_spmf]) simp
- text \<open>We rearrange the asserts\<close>
-  also have "\<dots> = TRY do {
-    PK \<leftarrow> KeyGen;
-    (C,calc_vec, \<sigma>) \<leftarrow> \<A> PK;
-    
-    (i, B, r_x, w_B) \<leftarrow> \<A>' \<sigma> PK C calc_vec;
-    _ :: unit \<leftarrow> assert_spmf (length PK = length calc_vec 
-                            \<and> C = fold (\<lambda> i acc. acc \<otimes>\<^bsub>G\<^sub>p\<^esub> PK!i ^\<^bsub>G\<^sub>p\<^esub> (calc_vec!i)) [0..<length PK] \<one>\<^bsub>G\<^sub>p\<^esub>);  
-    let \<phi> = E C calc_vec;
-    let \<phi>_i = poly \<phi> i;
-    let w_i = createWitness PK \<phi> i;
-    _ :: unit \<leftarrow> assert_spmf (i \<in> B \<and> \<phi>_i \<noteq> poly r_x i 
-                            \<and> valid_msg \<phi>_i w_i \<and> valid_batch_msg r_x w_B B
-                            \<and> VerifyEval PK C i \<phi>_i w_i \<and> VerifyEvalBatch PK C B r_x w_B);
-    return_spmf True
-  } ELSE return_spmf False"
-  proof -
-    have "do {
-    PK \<leftarrow> KeyGen;
-    (C,calc_vec, \<sigma>) \<leftarrow> \<A> PK;
-    _ :: unit \<leftarrow> assert_spmf (length PK = length calc_vec 
-                            \<and> C = fold (\<lambda> i acc. acc \<otimes>\<^bsub>G\<^sub>p\<^esub> PK!i ^\<^bsub>G\<^sub>p\<^esub> (calc_vec!i)) [0..<length PK] \<one>\<^bsub>G\<^sub>p\<^esub>);  
-    let \<phi> = E C calc_vec;
-    (i, B, r_x, w_B) \<leftarrow> \<A>' \<sigma> PK C calc_vec;
-    let \<phi>_i = poly \<phi> i;
-    let w_i = createWitness PK \<phi> i;
-    _ :: unit \<leftarrow> assert_spmf (i \<in> B \<and> \<phi>_i \<noteq> poly r_x i 
-                            \<and> valid_msg \<phi>_i w_i \<and> valid_batch_msg r_x w_B B
-                            \<and> VerifyEval PK C i \<phi>_i w_i \<and> VerifyEvalBatch PK C B r_x w_B);
-    return_spmf True
-    } = do {
-    PK \<leftarrow> KeyGen;
-    (C,calc_vec, \<sigma>) \<leftarrow> \<A> PK;
-    
-    (i, B, r_x, w_B) \<leftarrow> \<A>' \<sigma> PK C calc_vec;
-    _ :: unit \<leftarrow> assert_spmf (length PK = length calc_vec 
-                            \<and> C = fold (\<lambda> i acc. acc \<otimes>\<^bsub>G\<^sub>p\<^esub> PK!i ^\<^bsub>G\<^sub>p\<^esub> (calc_vec!i)) [0..<length PK] \<one>\<^bsub>G\<^sub>p\<^esub>);  
-    let \<phi> = E C calc_vec;
-    let \<phi>_i = poly \<phi> i;
-    let w_i = createWitness PK \<phi> i;
-    _ :: unit \<leftarrow> assert_spmf (i \<in> B \<and> \<phi>_i \<noteq> poly r_x i 
-                            \<and> valid_msg \<phi>_i w_i \<and> valid_batch_msg r_x w_B B
-                            \<and> VerifyEval PK C i \<phi>_i w_i \<and> VerifyEvalBatch PK C B r_x w_B);
-    return_spmf True
-    }"
-      using pull_down_assert_spmf_with_assert[of KeyGen \<A>] 
-      by (simp add: Let_def split_def)
-    then show ?thesis by argo
-  qed
-  text \<open>We unfold the game again into smaller sub games, so we can accumulate the rearranged assert 
-  as well.\<close>
-  also have "\<dots> = TRY do {
-    PK \<leftarrow> KeyGen;
-    TRY do {
-    (C,calc_vec, \<sigma>) \<leftarrow> \<A> PK;
-    TRY do {
-    (i, B, r_x, w_B) \<leftarrow> \<A>' \<sigma> PK C calc_vec;
-    TRY do {
-    _ :: unit \<leftarrow> assert_spmf (length PK = length calc_vec 
-                            \<and> C = fold (\<lambda> i acc. acc \<otimes>\<^bsub>G\<^sub>p\<^esub> PK!i ^\<^bsub>G\<^sub>p\<^esub> (calc_vec!i)) [0..<length PK] \<one>\<^bsub>G\<^sub>p\<^esub>);  
-    let \<phi> = E C calc_vec;
-    let \<phi>_i = poly \<phi> i;
-    let w_i = createWitness PK \<phi> i;
-    _ :: unit \<leftarrow> assert_spmf (i \<in> B \<and> \<phi>_i \<noteq> poly r_x i 
-                            \<and> valid_msg \<phi>_i w_i \<and> valid_batch_msg r_x w_B B
-                            \<and> VerifyEval PK C i \<phi>_i w_i \<and> VerifyEvalBatch PK C B r_x w_B);
-    return_spmf True
-    } ELSE return_spmf False
-    } ELSE return_spmf False 
-    } ELSE return_spmf False
-  } ELSE return_spmf False"
-  unfolding split_def Let_def 
-  by(fold try_bind_spmf_lossless2[OF lossless_return_spmf]) simp
-  text \<open>We accumulate the last assert\<close>
-  also have "\<dots> = TRY do {
-    PK \<leftarrow> KeyGen;
-    TRY do {
-    (C,calc_vec, \<sigma>) \<leftarrow> \<A> PK;
-    TRY do {
-    (i, B, r_x, w_B) \<leftarrow> \<A>' \<sigma> PK C calc_vec;
-    TRY do {
-    let \<phi> = E C calc_vec;
-    let \<phi>_i = poly \<phi> i;
-    let w_i = createWitness PK \<phi> i;
-    _ :: unit \<leftarrow> assert_spmf (length PK = length calc_vec 
-                            \<and> C = fold (\<lambda> i acc. acc \<otimes>\<^bsub>G\<^sub>p\<^esub> PK!i ^\<^bsub>G\<^sub>p\<^esub> (calc_vec!i)) [0..<length PK] \<one>\<^bsub>G\<^sub>p\<^esub>
-                            \<and> i \<in> B \<and> \<phi>_i \<noteq> poly r_x i 
-                            \<and> valid_msg \<phi>_i w_i \<and> valid_batch_msg r_x w_B B
-                            \<and> VerifyEval PK C i \<phi>_i w_i \<and> VerifyEvalBatch PK C B r_x w_B);
-    return_spmf True
-    } ELSE return_spmf False
-    } ELSE return_spmf False 
-    } ELSE return_spmf False
-  } ELSE return_spmf False"
-    unfolding Let_def
-    using assert_anding by presburger
-  text \<open>We fold the sub games together to one clean coherent game.\<close>
-  also have "\<dots> = TRY do {
-    PK \<leftarrow> KeyGen;
-    (C,calc_vec, \<sigma>) \<leftarrow> \<A> PK;
-    (i, B, r_x, w_B) \<leftarrow> \<A>' \<sigma> PK C calc_vec;
-    let \<phi> = E C calc_vec;
-    let \<phi>_i = poly \<phi> i;
-    let w_i = createWitness PK \<phi> i;
-    _ :: unit \<leftarrow> assert_spmf (length PK = length calc_vec 
-                            \<and> C = fold (\<lambda> i acc. acc \<otimes>\<^bsub>G\<^sub>p\<^esub> PK!i ^\<^bsub>G\<^sub>p\<^esub> (calc_vec!i)) [0..<length PK] \<one>\<^bsub>G\<^sub>p\<^esub>
-                            \<and> i \<in> B \<and> \<phi>_i \<noteq> poly r_x i 
-                            \<and> valid_msg \<phi>_i w_i \<and> valid_batch_msg r_x w_B B
-                            \<and> VerifyEval PK C i \<phi>_i w_i \<and> VerifyEvalBatch PK C B r_x w_B);
-    return_spmf True
-  } ELSE return_spmf False"
-   unfolding split_def Let_def 
-   by(fold try_bind_spmf_lossless2[OF lossless_return_spmf]) simp
- text \<open>Similarly to the prior lemma, we lastly want to make PK accessible in the assert statement and thus
-  we firstly unfold KeyGen to reveal the computation of PK.\<close>
-  also have "\<dots> = TRY do {
-    x :: nat \<leftarrow> sample_uniform (order G\<^sub>p);
-    let \<alpha> = of_int_mod_ring (int x);
-    PK \<leftarrow> return_spmf (map (\<lambda>t. \<^bold>g\<^bsub>G\<^sub>p\<^esub> ^\<^bsub>G\<^sub>p\<^esub> (\<alpha>^t)) [0..<max_deg+1]);
-    (C,calc_vec, \<sigma>) \<leftarrow> \<A> PK;
-    (i, B, r_x, w_B) \<leftarrow> \<A>' \<sigma> PK C calc_vec;
-    let \<phi> = E C calc_vec;
-    let \<phi>_i = poly \<phi> i;
-    let w_i = createWitness PK \<phi> i;
-    _ :: unit \<leftarrow> assert_spmf (length PK = length calc_vec 
-                            \<and> C = fold (\<lambda> i acc. acc \<otimes>\<^bsub>G\<^sub>p\<^esub> PK!i ^\<^bsub>G\<^sub>p\<^esub> (calc_vec!i)) [0..<length PK] \<one>\<^bsub>G\<^sub>p\<^esub>
-                            \<and> i \<in> B \<and> \<phi>_i \<noteq> poly r_x i 
-                            \<and> valid_msg \<phi>_i w_i \<and> valid_batch_msg r_x w_B B
-                            \<and> VerifyEval PK C i \<phi>_i w_i \<and> VerifyEvalBatch PK C B r_x w_B);
-       return_spmf True
-    } ELSE return_spmf False"
-    using key_gen_alt_def
-    by (smt (verit, ccfv_SIG) bind_spmf_assoc bind_spmf_cong)
-  text \<open>Secondly, we extract the definition of PK out of the spmf into a constant one.\<close>
-  also have "\<dots> = TRY do {
-    x :: nat \<leftarrow> sample_uniform (order G\<^sub>p);
-    let \<alpha> = of_int_mod_ring (int x);
-    let PK = map (\<lambda>t. \<^bold>g\<^bsub>G\<^sub>p\<^esub> ^\<^bsub>G\<^sub>p\<^esub> (\<alpha>^t)) [0..<max_deg+1];
-    (C,calc_vec, \<sigma>) \<leftarrow> \<A> PK;
-    (i, B, r_x, w_B) \<leftarrow> \<A>' \<sigma> PK C calc_vec;
-    let \<phi> = E C calc_vec;
-    let \<phi>_i = poly \<phi> i;
-    let w_i = createWitness PK \<phi> i;
-    _ :: unit \<leftarrow> assert_spmf (length PK = length calc_vec 
-                            \<and> C = fold (\<lambda> i acc. acc \<otimes>\<^bsub>G\<^sub>p\<^esub> PK!i ^\<^bsub>G\<^sub>p\<^esub> (calc_vec!i)) [0..<length PK] \<one>\<^bsub>G\<^sub>p\<^esub>
-                            \<and> i \<in> B \<and> \<phi>_i \<noteq> poly r_x i 
-                            \<and> valid_msg \<phi>_i w_i \<and> valid_batch_msg r_x w_B B
-                            \<and> VerifyEval PK C i \<phi>_i w_i \<and> VerifyEvalBatch PK C B r_x w_B);
-       return_spmf True
-    } ELSE return_spmf False"
-    using return_bind_spmf by meson
-  finally show ?thesis unfolding Let_def .
-qed
-
-text \<open>Proof Step 3:
-
-We show the equivalence of the content of the assert statements in the alt games i.e.
-assert content of knowledge_soundness_game_alt_def
-is equivalent to the 
-assert content of bind_game_knowledge_soundness_reduction_alt_def\<close>
-lemma asserts_are_equal: 
-  "length (map (\<lambda>t::nat. \<^bold>g ^\<^bsub>G\<^sub>p\<^esub> \<alpha> ^ t) [0::nat..<max_deg + (1::nat)]) = length calc_vec \<and>
-                      C =
-                      fold
-                       (\<lambda>(i::nat) acc::'a.
-                           acc \<otimes>\<^bsub>G\<^sub>p\<^esub> map (\<lambda>t::nat. \<^bold>g ^\<^bsub>G\<^sub>p\<^esub> \<alpha> ^ t) [0::nat..<max_deg + (1::nat)] ! i ^\<^bsub>G\<^sub>p\<^esub> calc_vec ! i)
-                       [0::nat..<length (map (\<lambda>t::nat. \<^bold>g ^\<^bsub>G\<^sub>p\<^esub> \<alpha> ^ t) [0::nat..<max_deg + (1::nat)])] \<one> \<and>
-                      i \<in> B \<and>
-                      valid_batch_msg r_x w_B B \<and>
-                      VerifyEvalBatch (map (\<lambda>t::nat. \<^bold>g ^\<^bsub>G\<^sub>p\<^esub> \<alpha> ^ t) [0::nat..<max_deg + (1::nat)]) C B r_x w_B \<and>
-                      poly r_x i \<noteq> poly (E C calc_vec) i 
-      \<longleftrightarrow> 
-  length (map (\<lambda>t::nat. \<^bold>g ^\<^bsub>G\<^sub>p\<^esub> \<alpha> ^ t) [0::nat..<max_deg + (1::nat)]) = length calc_vec \<and>
-                      C =
-                      fold
-                       (\<lambda>(i::nat) acc::'a.
-                           acc \<otimes>\<^bsub>G\<^sub>p\<^esub> map (\<lambda>t::nat. \<^bold>g ^\<^bsub>G\<^sub>p\<^esub> \<alpha> ^ t) [0::nat..<max_deg + (1::nat)] ! i ^\<^bsub>G\<^sub>p\<^esub> calc_vec ! i)
-                       [0::nat..<length (map (\<lambda>t::nat. \<^bold>g ^\<^bsub>G\<^sub>p\<^esub> \<alpha> ^ t) [0::nat..<max_deg + (1::nat)])] \<one> \<and>
-                      i \<in> B \<and>
-                      poly (E C calc_vec) i \<noteq> poly r_x i \<and>
-                      valid_msg (poly (E C calc_vec) i)
-                       (createWitness (map (\<lambda>t::nat. \<^bold>g ^\<^bsub>G\<^sub>p\<^esub> \<alpha> ^ t) [0::nat..<max_deg + (1::nat)]) (E C calc_vec) i) \<and>
-                      valid_batch_msg r_x w_B B \<and>
-                      VerifyEval (map (\<lambda>t::nat. \<^bold>g ^\<^bsub>G\<^sub>p\<^esub> \<alpha> ^ t) [0::nat..<max_deg + (1::nat)]) C i
-                       (poly (E C calc_vec) i)
-                       (createWitness (map (\<lambda>t::nat. \<^bold>g ^\<^bsub>G\<^sub>p\<^esub> \<alpha> ^ t) [0::nat..<max_deg + (1::nat)]) (E C calc_vec) i) \<and>
-                      VerifyEvalBatch (map (\<lambda>t::nat. \<^bold>g ^\<^bsub>G\<^sub>p\<^esub> \<alpha> ^ t) [0::nat..<max_deg + (1::nat)]) C B r_x w_B"
-  (is "?lhs \<longleftrightarrow> ?rhs")
-proof 
-  let ?PK = "(map (\<lambda>t. \<^bold>g\<^bsub>G\<^sub>p\<^esub> ^\<^bsub>G\<^sub>p\<^esub> (\<alpha>^t)) [0..<max_deg+1])"
-  let ?\<phi> = "Poly calc_vec"
-  
-  assume asm: ?lhs
-  show ?rhs
-  proof (intro conjI)
-    show "length (map (\<lambda>t::nat. \<^bold>g ^ \<alpha> ^ t) [0::nat..<max_deg + (1::nat)]) = length calc_vec"
-      using asm by blast
-    show C: "C =
-    fold (\<lambda>(i::nat) acc::'a. acc \<otimes> map (\<lambda>t::nat. \<^bold>g ^ \<alpha> ^ t) [0::nat..<max_deg + (1::nat)] ! i ^ calc_vec ! i)
-     [0::nat..<length (map (\<lambda>t::nat. \<^bold>g ^ \<alpha> ^ t) [0::nat..<max_deg + (1::nat)])] \<one>"
-      using asm by fast
-    show " i \<in> B"
-      using asm by blast
-    show "poly (E C calc_vec) i \<noteq> poly r_x i"
-      using asm by argo
-    show "valid_msg (poly (E C calc_vec) i) 
-     (createWitness (map (\<lambda>t::nat. \<^bold>g ^ \<alpha> ^ t) [0::nat..<max_deg + (1::nat)]) (E C calc_vec) i)"
-      proof -
-      have "g_pow_PK_Prod ?PK (\<psi>_of (Poly calc_vec) i) 
-      = \<^bold>g\<^bsub>G\<^sub>p\<^esub> ^\<^bsub>G\<^sub>p\<^esub> (poly (\<psi>_of (Poly calc_vec) i) \<alpha>)"
-      proof (rule g_pow_PK_Prod_correct)
-        show "degree (\<psi>_of (Poly calc_vec) i) \<le> max_deg"
-        proof (rule  le_trans[OF degree_q_le_\<phi>])
-          have "length calc_vec = max_deg +1"
-            using asm by force
-          moreover have "length (coeffs (Poly calc_vec)) \<le> length calc_vec"
-            by (simp add: length_strip_while_le)
-          ultimately show "degree (Poly calc_vec) \<le> max_deg"
-            using degree_eq_length_coeffs[of "Poly calc_vec"] by linarith
-        qed
-      qed
-      then show ?thesis 
-        unfolding valid_msg_def createWitness.simps Let_def
-        by simp
-    qed
-    show "valid_batch_msg r_x w_B B"
-      using asm by fast
-    show "VerifyEval (map (\<lambda>t::nat. \<^bold>g ^ \<alpha> ^ t) [0::nat..<max_deg + (1::nat)]) C i (poly (E C calc_vec) i)
-     (createWitness (map (\<lambda>t::nat. \<^bold>g ^ \<alpha> ^ t) [0::nat..<max_deg + (1::nat)]) (E C calc_vec) i)"
-     proof -
-      have length_calc_vec: "length calc_vec = max_deg +1"
-            using asm by force
-      moreover have "length (coeffs (Poly calc_vec)) \<le> length calc_vec"
-        by (simp add: length_strip_while_le)
-      ultimately have deg_poly_calc_vec_le_max_deg: "degree (Poly calc_vec) \<le> max_deg"
-        using degree_eq_length_coeffs[of "Poly calc_vec"] by linarith
-      
-      have 1: "(g_pow_PK_Prod (map (\<lambda>t. \<^bold>g ^\<^bsub>G\<^sub>p\<^esub> \<alpha> ^ t) [0..<max_deg + 1])
-        (\<psi>_of (Poly calc_vec) i))
-        = (\<^bold>g ^\<^bsub>G\<^sub>p\<^esub> poly (\<psi>_of (Poly calc_vec) i) \<alpha>)"
-      proof(rule  g_pow_PK_Prod_correct)
-        show "degree (\<psi>_of (Poly calc_vec) i) \<le> max_deg"
-          by (rule le_trans[OF degree_q_le_\<phi>])(fact deg_poly_calc_vec_le_max_deg)
-      qed
-
-      have 2: "map (\<lambda>t. \<^bold>g ^\<^bsub>G\<^sub>p\<^esub> \<alpha> ^ t) [0..<max_deg + 1] ! 1 = \<^bold>g ^\<^bsub>G\<^sub>p\<^esub> \<alpha>"
-        by (metis (no_types, lifting) One_nat_def add.commute d_pos diff_zero le_add_same_cancel1 le_zero_eq length_upt nth_map nth_upt plus_1_eq_Suc power_one_right zero_compare_simps(1))
-      
-      have 3: "C = (\<^bold>g ^\<^bsub>G\<^sub>p\<^esub> poly (Poly calc_vec) \<alpha>)"
-      proof -
-        have "(\<^bold>g ^\<^bsub>G\<^sub>p\<^esub> poly (Poly calc_vec) \<alpha>) 
-             = g_pow_PK_Prod (map (\<lambda>t. \<^bold>g ^\<^bsub>G\<^sub>p\<^esub> \<alpha> ^ t) [0..<max_deg + 1]) (Poly calc_vec)"
-          by (rule  g_pow_PK_Prod_correct[symmetric])(fact deg_poly_calc_vec_le_max_deg)
-        also have g_pow_to_fold: "\<dots> = fold (\<lambda>i acc. acc \<otimes>\<^bsub>G\<^sub>p\<^esub> (\<^bold>g\<^bsub>G\<^sub>p\<^esub> ^\<^bsub>G\<^sub>p\<^esub> (\<alpha>^i)) ^\<^bsub>G\<^sub>p\<^esub> (poly.coeff (Poly calc_vec) i)) [0..<Suc (degree (Poly calc_vec))] \<one>\<^bsub>G\<^sub>p\<^esub>"
-          by(rule g_pow_PK_Prod_to_fold)(fact deg_poly_calc_vec_le_max_deg)
-        also have "\<dots> 
-        =fold (\<lambda> i acc. acc \<otimes>\<^bsub>G\<^sub>p\<^esub> (\<^bold>g\<^bsub>G\<^sub>p\<^esub> ^\<^bsub>G\<^sub>p\<^esub> (\<alpha>^i)) ^\<^bsub>G\<^sub>p\<^esub> (calc_vec!i)) [0..<max_deg+1] \<one>\<^bsub>G\<^sub>p\<^esub>"
-        proof -
-          have "fold (\<lambda>i acc. acc \<otimes> (\<^bold>g ^\<^bsub>G\<^sub>p\<^esub> \<alpha> ^ i) ^\<^bsub>G\<^sub>p\<^esub> calc_vec ! i) [0..<max_deg + 1] \<one>
-              = fold (\<lambda>i acc. acc \<otimes> (\<^bold>g ^\<^bsub>G\<^sub>p\<^esub> \<alpha> ^ i) ^\<^bsub>G\<^sub>p\<^esub> calc_vec ! i) 
-                  ([0..<Suc (degree (Poly calc_vec))] @ [Suc (degree (Poly calc_vec))..<max_deg + 1]) 
-                  \<one>" 
-          proof -
-            have "Suc (degree (Poly calc_vec)) \<le> max_deg +1"
-              by (simp add: deg_poly_calc_vec_le_max_deg)
-            then show ?thesis
-              by (metis (no_types, lifting) nat_le_iff_add not_less not_less_eq_eq upt_add_eq_append zero_less_Suc)
-          qed
-          also have "\<dots> = fold (\<lambda>i acc. acc \<otimes> (\<^bold>g ^\<^bsub>G\<^sub>p\<^esub> \<alpha> ^ i) ^\<^bsub>G\<^sub>p\<^esub> calc_vec ! i) 
-                            [Suc (degree (Poly calc_vec))..<max_deg + 1]
-                            (fold (\<lambda>i acc. acc \<otimes> (\<^bold>g ^\<^bsub>G\<^sub>p\<^esub> \<alpha> ^ i) ^\<^bsub>G\<^sub>p\<^esub> calc_vec ! i) 
-                             [0..<Suc (degree (Poly calc_vec))] \<one>)"
-            by fastforce
-          also have "\<dots> = fold (\<lambda>i acc. acc \<otimes> (\<^bold>g ^\<^bsub>G\<^sub>p\<^esub> \<alpha> ^ i) ^\<^bsub>G\<^sub>p\<^esub> poly.coeff (Poly calc_vec) i) 
-                            [0..<Suc (degree (Poly calc_vec))] 
-                            \<one>"
-          proof -
-            have "fold (\<lambda>i acc. acc \<otimes> (\<^bold>g ^\<^bsub>G\<^sub>p\<^esub> \<alpha> ^ i) ^\<^bsub>G\<^sub>p\<^esub> calc_vec ! i) [0..<Suc (degree (Poly calc_vec))] \<one> 
-                = fold (\<lambda>i acc. acc \<otimes> (\<^bold>g ^\<^bsub>G\<^sub>p\<^esub> \<alpha> ^ i) ^\<^bsub>G\<^sub>p\<^esub> poly.coeff (Poly calc_vec) i) [0..<Suc (degree (Poly calc_vec))] \<one>" 
-            proof (rule List.fold_cong) 
-              show " \<And>x. x \<in> set [0..<Suc (degree (Poly calc_vec))] \<Longrightarrow>
-                       (\<lambda>acc. acc \<otimes> (\<^bold>g ^\<^bsub>G\<^sub>p\<^esub> \<alpha> ^ x) ^\<^bsub>G\<^sub>p\<^esub> calc_vec ! x) =
-                       (\<lambda>acc. acc \<otimes> (\<^bold>g ^\<^bsub>G\<^sub>p\<^esub> \<alpha> ^ x) ^\<^bsub>G\<^sub>p\<^esub> poly.coeff (Poly calc_vec) x)"
-              proof 
-                fix x::nat
-                fix acc::'a
-                assume asm: "x \<in> set [0..<Suc (degree (Poly calc_vec))]"
-                then have " calc_vec ! x = poly.coeff (Poly calc_vec) x"
-                  by (metis \<open>length calc_vec = max_deg + 1\<close> atLeastLessThan_iff coeff_Poly deg_poly_calc_vec_le_max_deg dual_order.trans less_Suc_eq_le nth_default_nth semiring_norm(174) set_upt)
-                then show " acc \<otimes> (\<^bold>g ^\<^bsub>G\<^sub>p\<^esub> \<alpha> ^ x) ^\<^bsub>G\<^sub>p\<^esub> calc_vec ! x = acc \<otimes> (\<^bold>g ^\<^bsub>G\<^sub>p\<^esub> \<alpha> ^ x) ^\<^bsub>G\<^sub>p\<^esub> poly.coeff (Poly calc_vec) x "
-                  by presburger
-              qed
-            qed simp+
-            moreover have "\<forall>init \<in> carrier G\<^sub>p. 
-                    fold (\<lambda>i acc. acc \<otimes> (\<^bold>g ^\<^bsub>G\<^sub>p\<^esub> \<alpha> ^ i) ^\<^bsub>G\<^sub>p\<^esub> calc_vec ! i) 
-                      [Suc (degree (Poly calc_vec))..<max_deg + 1] 
-                      init 
-                    = init"
-            proof 
-              fix init ::'a
-              assume init_in_carrier: "init \<in> carrier G\<^sub>p"
-              have "fold (\<lambda>i acc. acc \<otimes> (\<^bold>g ^\<^bsub>G\<^sub>p\<^esub> \<alpha> ^ i) ^\<^bsub>G\<^sub>p\<^esub> calc_vec ! i) 
-                      [Suc (degree (Poly calc_vec))..<max_deg + 1] 
-                      init = fold (\<lambda>i acc. acc \<otimes> \<one>) 
-                      [Suc (degree (Poly calc_vec))..<max_deg + 1] 
-                      init"
-              proof (rule List.fold_cong)
-                show " \<And>x. x \<in> set [Suc (degree (Poly calc_vec))..<max_deg + 1] \<Longrightarrow>
-                        (\<lambda>acc. acc \<otimes> (\<^bold>g ^\<^bsub>G\<^sub>p\<^esub> \<alpha> ^ x) ^\<^bsub>G\<^sub>p\<^esub> calc_vec ! x) = (\<lambda>acc. acc \<otimes> \<one>)"
-                proof 
-                  fix x::nat
-                  fix acc ::'a
-                  assume asm: "x \<in> set [Suc (degree (Poly calc_vec))..<max_deg + 1]"
-                  show "acc \<otimes> (\<^bold>g ^\<^bsub>G\<^sub>p\<^esub> \<alpha> ^ x) ^\<^bsub>G\<^sub>p\<^esub> calc_vec ! x = acc  \<otimes> \<one>"
-                  proof -
-                    have " calc_vec ! x = 0" using asm length_calc_vec
-                      by (smt (verit) add.commute coeff_Poly_eq in_set_conv_nth le_degree length_upt less_diff_conv not_less_eq_eq nth_default_eq_dflt_iff nth_upt order.refl trans_le_add2)
-                    then have "(\<^bold>g ^\<^bsub>G\<^sub>p\<^esub> \<alpha> ^ x) ^\<^bsub>G\<^sub>p\<^esub> calc_vec ! x = \<one>" by simp
-                    then show ?thesis by argo 
-                  qed
-                qed
-              qed simp+
-              also have "\<dots> = init" 
-              proof (induction max_deg)
-                case 0
-                then show ?case by fastforce
-              next
-                case (Suc max_deg)
-                have "fold (\<lambda>i acc. acc \<otimes> \<one>) [Suc (degree (Poly calc_vec))..<Suc max_deg + 1] init
-                = fold (\<lambda>i acc. acc \<otimes> \<one>) ([Suc (degree (Poly calc_vec))..<max_deg + 1] @ [Suc max_deg]) init"
-                  by (simp add: init_in_carrier)
-                also have "\<dots> = fold (\<lambda>i acc. acc \<otimes> \<one>) [Suc max_deg] (fold (\<lambda>i acc. acc \<otimes> \<one>) [Suc (degree (Poly calc_vec))..<max_deg + 1] init)"
-                  by force
-                also have "\<dots> = fold (\<lambda>i acc. acc \<otimes> \<one>) [Suc max_deg] init" using Suc.IH by argo
-                also have "\<dots> = init \<otimes> \<one>" by force
-                also have "\<dots> = init" by (simp add: init_in_carrier)
-                finally show ?case .
-              qed
-              finally show "fold (\<lambda>i acc. acc \<otimes> (\<^bold>g ^\<^bsub>G\<^sub>p\<^esub> \<alpha> ^ i) ^\<^bsub>G\<^sub>p\<^esub> calc_vec ! i) 
-                      [Suc (degree (Poly calc_vec))..<max_deg + 1] 
-                      init 
-                   = init" .
-            qed
-            ultimately show ?thesis
-              by (metis (no_types, lifting) G\<^sub>p.generator_closed G\<^sub>p.int_pow_closed \<open>\<^bold>g ^\<^bsub>G\<^sub>p\<^esub> poly (Poly calc_vec) \<alpha> = g_pow_PK_Prod (map (\<lambda>t. \<^bold>g ^\<^bsub>G\<^sub>p\<^esub> \<alpha> ^ t) [0..<max_deg + 1]) (Poly calc_vec)\<close> g_pow_to_fold)
-          qed
-          finally show ?thesis by presburger
-        qed
-        also have "\<dots> 
-        =fold (\<lambda> i acc. acc \<otimes>\<^bsub>G\<^sub>p\<^esub> (map (\<lambda>t. \<^bold>g\<^bsub>G\<^sub>p\<^esub> ^\<^bsub>G\<^sub>p\<^esub> (\<alpha>^t)) [0..<max_deg+1])!i ^\<^bsub>G\<^sub>p\<^esub> (calc_vec!i)) [0..<max_deg+1] \<one>\<^bsub>G\<^sub>p\<^esub>"
-        proof(rule List.fold_cong)
-          show "\<one> = \<one>" by simp
-          show "[0..<max_deg + 1] = [0..<max_deg + 1]" by simp
-          show "\<And>x. x \<in> set [0..<max_deg + 1] \<Longrightarrow>
-           (\<lambda>acc. acc \<otimes> (\<^bold>g ^\<^bsub>G\<^sub>p\<^esub> \<alpha> ^ x) ^\<^bsub>G\<^sub>p\<^esub> calc_vec ! x) =
-           (\<lambda>acc. acc \<otimes> map (\<lambda>t. \<^bold>g ^\<^bsub>G\<^sub>p\<^esub> \<alpha> ^ t) [0..<max_deg + 1] ! x ^\<^bsub>G\<^sub>p\<^esub> calc_vec ! x)"
-          proof 
-            fix x::nat 
-            fix acc :: 'a
-            assume asm: "x \<in> set [0..<max_deg + 1]"
-            show " acc \<otimes> (\<^bold>g ^\<^bsub>G\<^sub>p\<^esub> \<alpha> ^ x) ^\<^bsub>G\<^sub>p\<^esub> calc_vec ! x 
-                 = acc \<otimes> map (\<lambda>t. \<^bold>g ^\<^bsub>G\<^sub>p\<^esub> \<alpha> ^ t) [0..<max_deg + 1] ! x ^\<^bsub>G\<^sub>p\<^esub> calc_vec ! x"
-              using PK_i[symmetric] asm
-              by (metis Suc_eq_plus1 atLeastLessThan_iff less_Suc_eq_le set_upt)
-          qed
-        qed
-        also have "\<dots> = C" 
-          using asm by fastforce
-        finally show ?thesis ..
-      qed
-      show ?thesis
-      unfolding VerifyEval_def createWitness.simps Let_def g_pow_PK_Prod_correct 3 2 1 E.simps
-      using eq_on_e[of "(Poly calc_vec)" i \<alpha>] by blast
-  qed
-    show "VerifyEvalBatch (map (\<lambda>t::nat. \<^bold>g ^ \<alpha> ^ t) [0::nat..<max_deg + (1::nat)]) C B r_x w_B"
-      using asm by linarith
-  qed 
-qed argo
-
-text \<open>Proof step 4:\<close>
-
-text \<open>From the last three steps, we conclude that the know,ledge_soundness_game is the same game as 
-the evaluation binding game for the extended reduction adversary.\<close>
-theorem knowledge_soundness_game_eq_bind_game_knowledge_soundness_reduction_ext: 
-  "knowledge_soundness_game E \<A> \<A>' = bind_game (knowledge_soundness_reduction_ext E \<A> \<A>')"
-  unfolding knowledge_soundness_game_alt_def 
-            bind_game_knowledge_soundness_reduction_alt_def
-            Let_def
-  using asserts_are_equal by simp
-
-text \<open>Proof Step 5:
-
-We overestimate the probability of winning the evaluation binding game with the extended adversary 
-by winning it with the normal adversary.\<close>
-lemma overestimate_reductions: "spmf (bind_game (knowledge_soundness_reduction_ext E \<A> \<A>')) True 
-  \<le> spmf (bind_game (knowledge_soundness_reduction E \<A> \<A>')) True"
-proof -
-   note [simp] = Let_def split_def
-
-   text \<open>We extend the evaluation binding game with the extended reduction adversary to a complete 
-   game.\<close>
-   have w_assert_ext: "bind_game (knowledge_soundness_reduction_ext E \<A> \<A>') = TRY do {
-    PK \<leftarrow> KeyGen;
-    (C,calc_vec, \<sigma>) \<leftarrow> \<A> PK;
-    _ :: unit \<leftarrow> assert_spmf (length PK = length calc_vec 
-                            \<and> C = fold (\<lambda> i acc. acc \<otimes>\<^bsub>G\<^sub>p\<^esub> PK!i ^\<^bsub>G\<^sub>p\<^esub> (calc_vec!i)) [0..<length PK] \<one>\<^bsub>G\<^sub>p\<^esub>);  
-    let \<phi> = E C calc_vec;
-    (i, B, r_x, w_B) \<leftarrow> \<A>' \<sigma> PK C calc_vec;
-    let \<phi>_i = poly \<phi> i;
-    let w_i = createWitness PK \<phi> i;
-    _ :: unit \<leftarrow> assert_spmf (i \<in> B \<and> \<phi>_i \<noteq> poly r_x i \<and> valid_msg \<phi>_i w_i \<and> valid_batch_msg r_x w_B B); 
-    let b = VerifyEval PK C i \<phi>_i w_i;
-    let b' = VerifyEvalBatch PK C B r_x w_B;
-    _::unit \<leftarrow> assert_spmf (b \<and> b');
-    return_spmf True} ELSE return_spmf False"
-     unfolding bind_game_alt_def knowledge_soundness_reduction_ext_def 
-     by (simp add: split_def Let_def)
-
-   text \<open>We extend the evaluation binding game with the normal reduction adversary to a complete 
-   game.\<close>
-   have wo_assert_ext: "bind_game (knowledge_soundness_reduction E \<A> \<A>') = TRY do {
-    PK \<leftarrow> KeyGen;
-    (C,calc_vec, \<sigma>) \<leftarrow> \<A> PK;
-    let \<phi> = E C calc_vec;
-    (i, B, r_x, w_B) \<leftarrow> \<A>' \<sigma> PK C calc_vec;
-    let \<phi>_i = poly \<phi> i;
-    let w_i = createWitness PK \<phi> i;
-    _ :: unit \<leftarrow> assert_spmf (i \<in> B \<and> \<phi>_i \<noteq> poly r_x i \<and> valid_msg \<phi>_i w_i \<and> valid_batch_msg r_x w_B B); 
-    let b = VerifyEval PK C i \<phi>_i w_i;
-    let b' = VerifyEvalBatch PK C B r_x w_B;
-    _::unit \<leftarrow> assert_spmf (b \<and> b');
-    return_spmf True} ELSE return_spmf False"
-     unfolding bind_game_alt_def knowledge_soundness_reduction_def 
-     by (simp add: split_def Let_def)
-
-  text \<open>We show the thesis in ennreal, which implies the plain thesis\<close>
-  have "ennreal (spmf (bind_game (knowledge_soundness_reduction_ext E \<A> \<A>')) True) 
-    \<le> ennreal (spmf (bind_game (knowledge_soundness_reduction E \<A> \<A>')) True)"
-    unfolding w_assert_ext wo_assert_ext
-    apply (simp add: spmf_try_spmf ennreal_spmf_bind)
-    apply (rule nn_integral_mono)+
-    apply (simp add: assert_spmf_def)
-    apply (simp add: measure_spmf.emeasure_eq_measure)
-    done
-    
-  then show ?thesis by simp
-qed
-  
-text \<open>Proof Step 6:
-
-Finally we put everything together:
+text \<open>Finally we put everything together:
 we conclude that for every efficient adversary in the AGM the advantage of winning the 
 knowledge soundness game is less equal to breaking the t-BSDH assumption.\<close>
 theorem knowledge_soundness: 
-  "knowledge_soundness_game_advantage E \<A> \<A>' 
-  \<le> t_BSDH.advantage (reduction (knowledge_soundness_reduction E \<A> \<A>'))"
-  using evaluation_binding[of "knowledge_soundness_reduction E \<A> \<A>'"]
-    overestimate_reductions[of \<A> \<A>']
-  unfolding bind_advantage_def knowledge_soundness_game_advantage_def 
-  unfolding knowledge_soundness_game_eq_bind_game_knowledge_soundness_reduction_ext
-  by linarith
+  "spmf (knowledge_soundness_game_AGM \<A>1 \<A>2 E) True 
+  \<le> t_BSDH.advantage (reduction (ks_to_eval_bind_reduction \<A>1 \<A>2 E))"
+  using  ks_game_to_eval_bind_game
+  using evaluation_binding[of "ks_to_eval_bind_reduction \<A>1 \<A>2 E"]
+  unfolding bind_advantage_def
+  using landau_o.R_trans by blast
 
 end
 
